Kruskal/Correctness copy.lean
@@ -1,0 +1,1862 @@
+-- import Mathlib
+import Kruskal.Basic
+-- import Kruskal.Lists
+import Kruskal.Tantow
+
+set_option maxHeartbeats 10000000
+
+-- set_option pp.all true
+
+namespace Kruskal
+
+
+variable {m n : Nat} {α β : Type}
+
+open SimpleGraph
+
+def SimpleGraph.IsSpanningTree (G : SimpleGraph α) (H : SimpleGraph α) : Prop := H ≤ G ∧ H.IsAcyclic ∧ (∀ (x y : α), G.Reachable x y ↔ H.Reachable x y)
+
+theorem spanninTree_connected_iff_connected (G : SimpleGraph α) (H : SimpleGraph α) (h : SimpleGraph.IsSpanningTree G H) : G.Connected ↔ H.Connected := by
+  simp [SimpleGraph.connected_iff_exists_forall_reachable]
+  simp [SimpleGraph.IsSpanningTree] at h
+  rcases h with ⟨_, _, h⟩
+  simp [h]
+
+theorem nodeList_of_edgeList_helper_nonempty {nodeList : List node} (edgeList : List edge) : nodeList ≠ [] → nodeList_of_edgeList_helper edgeList nodeList ≠ [] := by
+  intro h'
+  induction edgeList generalizing nodeList with
+  | nil =>
+    simp [nodeList_of_edgeList_helper, h']
+  | cons e edgeList ih =>
+    by_cases h_eq : e.node1 = e.node2
+    · simp [nodeList_of_edgeList_helper, h_eq]
+      by_cases h_in : { id := e.node2 } ∈ nodeList
+      · simp [h_in]
+        apply ih h'
+      · simp [h_in]
+        apply ih
+        · simp
+    · simp [nodeList_of_edgeList_helper]
+      by_cases h_in₁ : { id := e.node1 } ∈ nodeList
+      · by_cases h_in₂ : { id := e.node2 } ∈ nodeList
+        · simp [h_in₁, h_in₂]
+          apply ih h'
+        · simp [h_in₁, h_in₂]
+          apply ih
+          · simp
+      · by_cases h_in₂ : { id := e.node2 } ∈ nodeList
+        · simp [h_in₁, h_in₂]
+          apply ih
+          · simp
+        · simp [h_in₁, h_in₂]
+          apply ih
+          · simp
+
+theorem nodeList_of_edgeList_nonempty (edgeList : List edge) (h : edgeList ≠ []) : nodeList_of_edgeList edgeList ≠ [] := by
+  cases edgeList with
+  | nil =>
+    simp at h
+  | cons e edgeList =>
+    simp [nodeList_of_edgeList, nodeList_of_edgeList_helper]
+    by_cases h_eq : e.node1 = e.node2
+    · simp [h_eq, nodeList_of_edgeList_helper_nonempty]
+    · simp [nodeList_of_edgeList_helper_nonempty]
+
+def nodeList_of_edgeList_max (edgeList : List edge) (h : edgeList ≠ []) : node := (nodeList_of_edgeList edgeList).max (nodeList_of_edgeList_nonempty edgeList h)
+
+def fin_of_edgeList (edgeList : List edge) (h : edgeList ≠ []) : Type := Fin (nodeList_of_edgeList_max edgeList h).id.succ
+
+def SimpleGraph_of_edgeList (edgeList : List edge) (h : edgeList ≠ []) : SimpleGraph (fin_of_edgeList edgeList h) where
+  Adj (a b) := ∃ e ∈ edgeList, (e.node1 = a.val ∧ e.node2 = b.val) ∨ (e.node1 = b.val ∧ e.node2 = a.val)
+  symm := by
+    simp [Symmetric]
+    intro a b e h_e_in h_adj
+    refine ⟨e, h_e_in, h_adj.symm⟩
+  loopless := by
+    simp [irrefl_def]
+    intro a e h_e h_eq₁ h_eq₂
+    have h_lt := e.nodesLt
+    simp [h_eq₁, h_eq₂] at h_lt
+
+def SimpleGraph_of_n_of_edgeList (n : Nat) (edgeList : List edge) (h : edgeList ≠ []) (h_eq : n = (nodeList_of_edgeList_max edgeList h).id.succ) : SimpleGraph (Fin n) :=
+  let G := SimpleGraph_of_edgeList edgeList h
+  let Adj := fun (a b : Fin n) => G.Adj ⟨a, by rw [← h_eq]; exact a.isLt⟩ ⟨b, by rw [← h_eq]; exact b.isLt⟩
+  have symm : Symmetric Adj := by
+    simp [Symmetric, Adj]
+    intro a b
+    have h_symm := G.symm
+    simp only [Symmetric] at h_symm
+    exact h_symm (x := ⟨a, by rw [← h_eq]; exact a.isLt⟩) (y := ⟨b, by rw [← h_eq]; exact b.isLt⟩)
+  have loopless : Std.Irrefl Adj := by
+    simp [irrefl_def, Adj]
+  ⟨Adj, symm, loopless⟩
+
+theorem connected_component_of_init_unionFind_of_id_eq_id {nodeList : List node} {h_nodup : nodeList.Nodup} {id : Nat} {h : ∃ x ∈ nodeList, x.id = id} : connected_component_of_unionFind_of_id (init_unionFind nodeList h_nodup) id h = id := by
+  simp [init_unionFind]
+  by_cases h_nonempty : nodeList ≠ []
+  · simp [h_nonempty]
+    simp [connected_component_of_unionFind_of_id]
+    have h_ex : ∃ y ∈ (init_unionFind.linkList nodeList (by simp [h_nonempty])), (fun x => x.nodeId = id) y := by
+      let uF := init_unionFind nodeList h_nodup
+      have h_linkList_eq : uF.linkList = (init_unionFind.linkList nodeList (by simp [h_nonempty])) := by
+        simp [uF, init_unionFind, h_nonempty]
+      simp [← h_linkList_eq]
+      rcases h with ⟨z, h_z_in, h_z_id_eq⟩
+      have h_matching_nodeId := uF.matching_nodeId z h_z_in
+      simp [ExistsUnique, h_z_id_eq] at h_matching_nodeId
+      rcases h_matching_nodeId with ⟨y, h_y, h_unique⟩
+      refine ⟨y, ?_⟩
+      simp [h_y]
+    set x := List.choose (fun x => x.nodeId = id) (init_unionFind.linkList nodeList (by simp [h_nonempty])) h_ex with h_x
+    simp [← h_x]
+    have h_x_in := List.choose_mem (fun x => x.nodeId = id) (init_unionFind.linkList nodeList (by simp [h_nonempty])) h_ex
+    simp [← h_x] at h_x_in
+    simp [init_unionFind.linkList] at h_x_in
+    have h_x_prop := List.choose_property (fun x => x.nodeId = id) (init_unionFind.linkList nodeList (by simp [h_nonempty])) h_ex
+    simp [← h_x] at h_x_prop
+    have h_x_selfcon := init_unionFind.linkList.helper_all_self_connected nodeList nodeList (by simp [h_nonempty]) x h_x_in
+    rw [connected_component_of_unionFind_of_unionFindLink]
+    simp [h_x_selfcon.symm, h_x_prop]
+  · simp at h_nonempty
+    simp [h_nonempty] at h
+
+theorem kruskal_helper_nonempty
+  {edgeList : List edge}
+  {nodeList : List node}
+  {uF : unionFind nodeList}
+  {edgesSoFar : List edge}
+  {h_matching_edge : matching_edge edgeList nodeList}
+  {h_nodup : nodeList.Nodup}
+  : edgesSoFar ≠ [] → kruskal_helper edgeList nodeList uF edgesSoFar h_matching_edge h_nodup ≠ [] := by
+  intro h_nonempty
+  induction edgeList generalizing uF edgesSoFar with
+  | nil =>
+    simp [kruskal_helper, h_nonempty]
+  | cons e edgeList ih =>
+    simp [kruskal_helper, update_unionFind]
+    apply ih
+    simp [update_edgesSoFar]
+    split_ifs
+    · exact h_nonempty
+    · simp
+
+theorem kruskal_nonempty (edgeList : List edge) (h : edgeList ≠ []) : kruskal_of_edgeList edgeList ≠ [] := by
+  simp [kruskal_of_edgeList]
+  unfold kruskal
+  -- simp [kruskal]
+  -- set edgeListSorted := edgeList.mergeSort with h_edgeListSorted
+  cases edgeList with
+  | nil =>
+    simp at h
+  | cons e edgeList =>
+    simp
+    -- simp [] at h_edgeListSorted
+    have h_split := List.mergeSort_cons (α := edge) (le := fun a b => decide (a ≤ b)) (by simp; exact edge_Preorder.le_trans) (by simp; exact edge_LinearOrder.le_total) e edgeList
+    rcases h_split with ⟨l₁, l₂, h_split⟩
+    simp [h_split]
+    cases l₁ with
+    | nil =>
+      simp [kruskal_helper]
+      simp [connected_component_of_init_unionFind_of_id_eq_id]
+      exact kruskal_helper_nonempty (by simp [update_edgesSoFar, ne_of_lt e.nodesLt])
+    | cons f l₁ =>
+      simp [kruskal_helper]
+      simp [connected_component_of_init_unionFind_of_id_eq_id]
+      exact kruskal_helper_nonempty (by simp [update_edgesSoFar, ne_of_lt f.nodesLt])
+
+def SimpleGraph_of_kruskal (edgeList : List edge) (h : edgeList ≠ []) := SimpleGraph_of_n_of_edgeList (nodeList_of_edgeList_max (kruskal_of_edgeList edgeList) _).id.succ (kruskal_of_edgeList edgeList) (kruskal_nonempty edgeList h) (rfl)
+
+theorem kruskal_helper_sublist {edgeList : List edge} {nodeList : List node} {uF : unionFind nodeList} {edgesSoFar : List edge} {h_matching_edge : matching_edge edgeList nodeList} {h_nodup : nodeList.Nodup} : ∀ e ∈ kruskal_helper edgeList nodeList uF edgesSoFar h_matching_edge h_nodup, e ∈ edgeList ∨ e ∈ edgesSoFar := by
+  induction edgeList, uF, edgesSoFar, h_matching_edge using kruskal_helper.induct with
+  | case1 uF edgesSoFar h_matching_edge =>
+    simp [kruskal_helper]
+  | case2 uF edgesSoFar e es h_matching_edge h_ex1 x h_ex2 y h_matching_edge' h_self_con1 h_self_con2 updated_uF updated_edgesSoFar ih =>
+    simp [kruskal_helper]
+    simp only [updated_uF, updated_edgesSoFar, x, y] at ih
+    by_cases h_eq : x = y
+    · simp [x, y] at h_eq
+      simp [update_edgesSoFar, h_eq]
+      simp [update_edgesSoFar, h_eq] at ih
+      grind
+    · simp [x, y] at h_eq
+      simp [update_edgesSoFar, h_eq]
+      simp [update_edgesSoFar, h_eq] at ih
+      grind
+
+theorem kruskal_sublist {edgeList : List edge} {nodeList : List node} {h_matching_edge : matching_edge edgeList nodeList} {h_nodup : nodeList.Nodup} : ∀ e ∈ kruskal edgeList nodeList h_matching_edge h_nodup, e ∈ edgeList := by
+  simp [kruskal]
+  intro e h_e_in
+  have h := kruskal_helper_sublist e h_e_in
+  simp at h
+  exact h
+
+theorem kruskal_helper.edgesSoFar_append
+  {edgeList : List edge}
+  {nodeList : List node}
+  {uF : unionFind nodeList}
+  {edgesSoFar₁ edgesSoFar₂ : List edge}
+  {h_matching_edge : matching_edge edgeList nodeList}
+  {h_nodup : nodeList.Nodup}
+  : kruskal_helper edgeList nodeList uF (edgesSoFar₁ ++ edgesSoFar₂) h_matching_edge h_nodup = kruskal_helper edgeList nodeList uF edgesSoFar₁ h_matching_edge h_nodup ++ edgesSoFar₂ := by
+  set edgesSoFar := edgesSoFar₁ ++ edgesSoFar₂ with h_edgesSoFar
+  revert h_edgesSoFar
+  induction edgeList, uF, edgesSoFar, h_matching_edge using kruskal_helper.induct nodeList generalizing edgesSoFar₁ with
+  | case1 uF edgesSoFar h_matching_edge =>
+    simp [kruskal_helper]
+  | case2 uF edgesSoFar e es h_matching_edge h_ex1 x h_ex2 y h_matching_edge' h_self_con1 h_self_con2 updated_uF updated_edgesSoFar =>
+    rename_i edgesSoFar' ih -- strange aber funktioniert so
+    intro h_edgesSoFar'
+    simp [updated_edgesSoFar, h_edgesSoFar'] at ih
+    simp [kruskal_helper]
+    have ih := ih (edgesSoFar₁ := update_edgesSoFar edgesSoFar₁ e x y )
+    by_cases h_eq : x = y
+    · simp [x, y] at h_eq
+      simp [update_edgesSoFar, h_eq]
+      simp [update_edgesSoFar] at ih
+      grind
+    · simp [x, y] at h_eq
+      simp [update_edgesSoFar, h_eq]
+      simp [update_edgesSoFar] at ih
+      grind
+
+theorem kruskal_helper.edgeList_append {edgeList₁ edgeList₂ : List edge} {nodeList : List node} {uF : unionFind nodeList} {edgesSoFar : List edge} {h_matching_edge : matching_edge (edgeList₁ ++ edgeList₂) nodeList} {h_matching_edge₁ : matching_edge edgeList₁ nodeList} {h_matching_edge₂ : matching_edge edgeList₂ nodeList} {h_nodup : nodeList.Nodup} : ∃ (uF' : unionFind nodeList), kruskal_helper (edgeList₁ ++ edgeList₂) nodeList uF edgesSoFar h_matching_edge h_nodup = kruskal_helper edgeList₂ nodeList uF' ((kruskal_helper edgeList₁ nodeList uF [] h_matching_edge₁ h_nodup) ++ edgesSoFar) h_matching_edge₂ h_nodup := by
+  induction edgeList₁ generalizing uF edgesSoFar with
+  | nil =>
+    simp
+    have h_empty : kruskal_helper [] nodeList uF [] h_matching_edge₁ h_nodup = [] := by
+      simp [kruskal_helper]
+    simp [h_empty]
+    refine ⟨uF, rfl⟩
+  | cons e edgeList₁ ih =>
+    simp [kruskal_helper]
+    simp [matching_edge] at h_matching_edge₁
+    by_cases h_eq : connected_component_of_unionFind_of_id uF e.node1 (by grind) = connected_component_of_unionFind_of_id uF e.node2 (by grind)
+    · simp [update_unionFind, h_eq]
+      have h : [e] = [] ++ [e] := by
+        simp
+      simp [update_edgesSoFar]
+      exact ih
+    · set uF' := update_unionFind uF (connected_component_of_unionFind_of_id uF e.node1 (by grind)) (connected_component_of_unionFind_of_id uF e.node2 (by grind)) _ _
+      simp [matching_edge] at h_matching_edge
+      have ih := ih (uF := uF') (edgesSoFar := e :: edgesSoFar) (h_matching_edge₁ := h_matching_edge₁.right) (h_matching_edge := by simp [matching_edge]; exact h_matching_edge.right)
+      rcases ih with ⟨uF'', ih⟩
+      simp [update_edgesSoFar, h_eq, ih]
+      have h_nil_append : [e] = [] ++ [e] := by
+        simp
+      rw [h_nil_append]
+      simp only [kruskal_helper.edgesSoFar_append]
+      simp
+      refine ⟨uF'', rfl⟩
+
+theorem kruskal_helper_not_con_invariant
+  {edgeList : List edge}
+  {nodeList : List node}
+  {uF : unionFind nodeList}
+  {edgesSoFar : List edge}
+  {h_matching_edge : matching_edge edgeList nodeList}
+  {h_nodup : nodeList.Nodup}
+  {z : node}
+  (h_edgeList_not_con : ∀ e ∈ edgeList, ¬(e.node1 = z.id ∨ e.node2 = z.id))
+  (h_uF_not_con : ∀ uFL ∈ uF.linkList, uFL.ccId = z.id ↔ uFL.nodeId = z.id)
+  : ∃ (uF' : unionFind nodeList), kruskal_helper edgeList nodeList uF edgesSoFar h_matching_edge h_nodup = kruskal_helper [] nodeList uF' ((kruskal_helper edgeList nodeList uF [] h_matching_edge h_nodup) ++ edgesSoFar) (by simp [matching_edge]) h_nodup ∧ ∀ uFL ∈ uF'.linkList, uFL.ccId = z.id ↔ uFL.nodeId = z.id := by
+  induction edgeList with
+  | nil =>
+    simp [kruskal_helper]
+    refine ⟨uF, h_uF_not_con⟩
+  | cons e edgeList ih =>
+    simp only [List.mem_cons, forall_eq_or_imp] at h_edgeList_not_con
+    set eSF := kruskal_helper (e :: edgeList) nodeList uF [] h_matching_edge h_nodup ++ edgesSoFar
+    set k := kruskal_helper (e :: edgeList) nodeList uF edgesSoFar h_matching_edge h_nodup
+    simp [kruskal_helper]
+    simp [eSF, k]
+    constructor
+    · have h : edgesSoFar = [] ++ edgesSoFar := by
+        simp
+      rw [h]
+      exact kruskal_helper.edgesSoFar_append
+    · refine ⟨uF, h_uF_not_con⟩
+
+theorem connected_component_of_unionFind_of_id_not_con
+  {nodeList : List node}
+  {uF : unionFind nodeList}
+  {z : node}
+  (h_z_in : z ∈ nodeList)
+  (h_uF_not_con : ∀ uFL ∈ uF.linkList, uFL.ccId = z.id ↔ uFL.nodeId = z.id)
+  : ∀ (x : node), (h_x_in : x ∈ nodeList) → connected_component_of_unionFind_of_id uF x.id ⟨x, h_x_in, rfl⟩ = z.id ↔ x = z := by
+  intro x h_x_in
+  constructor
+  · simp [connected_component_of_unionFind_of_id]
+    have h_ex_uFLx : ∃ a ∈ uF.linkList, (fun y => y.nodeId = x.id) a := by
+      have h := uF.matching_nodeId x h_x_in
+      simp [ExistsUnique] at h
+      rcases h with ⟨a, h_a, _⟩
+      grind
+    set uFLx := List.choose (fun y => y.nodeId = x.id) uF.linkList h_ex_uFLx with h_uFLx
+    have h_uFLx_prop := List.choose_property (fun y => y.nodeId = x.id) uF.linkList h_ex_uFLx
+    have h_uFLx_in := List.choose_mem (fun y => y.nodeId = x.id) uF.linkList h_ex_uFLx
+    simp_all [← h_uFLx]
+    by_cases h_uFLx_self_con : uFLx.ccId = uFLx.nodeId
+    · rw [connected_component_of_unionFind_of_unionFindLink]
+      simp [← h_uFLx_self_con]
+      intro h_eq
+      have h := (h_uF_not_con uFLx h_uFLx_in).mp h_eq
+      cases x
+      cases z
+      simp [h] at h_uFLx_prop
+      simp [h_uFLx_prop.symm]
+    · have h_goal : ∀ (uFL : unionFindLink nodeList) (h_in : uFL ∈ uF.linkList), connected_component_of_unionFind_of_unionFindLink uF uFL h_in = z.id → uFL.nodeId = z.id := by
+        intro uFL h_uFL_in
+        induction uFL, h_uFL_in using connected_component_of_unionFind_of_unionFindLink.induct with
+        | case1 uFL h_uFL_in h_uFL_self_con =>
+          rw [connected_component_of_unionFind_of_unionFindLink]
+          simp [h_uFL_self_con]
+        | case2 uFL h_uFL_in h_uFL_not_self_con uFLy h_uFLy_in h_rank_lt ih =>
+          rw [connected_component_of_unionFind_of_unionFindLink]
+          simp [h_uFL_not_self_con]
+          intro h_id
+          have h_uFLx_prop := List.choose_property (fun y => y.nodeId = uFL.ccId) uF.linkList (by grind)
+          simp [h_id, uFLy, h_uFLx_prop] at ih
+          exact (h_uF_not_con uFL h_uFL_in).mp ih
+      intro h_eq
+      have h := h_goal uFLx h_uFLx_in h_eq
+      simp [h_uFLx_prop] at h
+      cases x
+      cases z
+      simp at h
+      simp [h]
+  · intro h_eq
+    simp [h_eq, connected_component_of_unionFind_of_id]
+    have h_ex_uFLz : ∃ a ∈ uF.linkList, (fun x => x.nodeId = z.id) a := by
+      have h := uF.matching_nodeId z h_z_in
+      simp [ExistsUnique] at h
+      rcases h with ⟨a, h_a, _⟩
+      grind
+    set uFLz := List.choose (fun x => x.nodeId = z.id) uF.linkList h_ex_uFLz with h_uFLz
+    have h_uFLz_prop := List.choose_property (fun x => x.nodeId = z.id) uF.linkList h_ex_uFLz
+    have h_uFLz_in := List.choose_mem (fun x => x.nodeId = z.id) uF.linkList h_ex_uFLz
+    simp [← h_uFLz] at *
+    rw [connected_component_of_unionFind_of_unionFindLink]
+    simp [h_uFLz_prop, (h_uF_not_con uFLz h_uFLz_in)]
+
+theorem kruskal_helper_not_con_invariant_append
+  {edgeList₁ edgeList₂ : List edge}
+  {nodeList : List node}
+  {uF : unionFind nodeList}
+  {edgesSoFar : List edge}
+  {h_matching_edge : matching_edge (edgeList₁ ++ edgeList₂) nodeList}
+  {h_nodup : nodeList.Nodup}
+  {z : node}
+  (h_z_in : z ∈ nodeList)
+  (h_edgeList_not_con : ∀ e ∈ edgeList₁, ¬(e.node1 = z.id ∨ e.node2 = z.id))
+  (h_uF_not_con : ∀ uFL ∈ uF.linkList, uFL.ccId = z.id ↔ uFL.nodeId = z.id)
+  : ∃ (uF' : unionFind nodeList), kruskal_helper (edgeList₁ ++ edgeList₂) nodeList uF edgesSoFar h_matching_edge h_nodup = kruskal_helper edgeList₂ nodeList uF' ((kruskal_helper edgeList₁ nodeList uF [] (by simp [matching_edge] at h_matching_edge; simp [matching_edge]; grind) h_nodup) ++ edgesSoFar) (by simp [matching_edge] at h_matching_edge; simp [matching_edge]; grind) h_nodup ∧ ∀ uFL ∈ uF'.linkList, uFL.ccId = z.id ↔ uFL.nodeId = z.id := by
+  induction edgeList₁ generalizing uF edgesSoFar with
+  | nil =>
+    simp [kruskal_helper]
+    refine ⟨uF, rfl, h_uF_not_con⟩
+  | cons e edgeList₁ ih =>
+    simp only [List.mem_cons, forall_eq_or_imp] at h_edgeList_not_con
+    simp [kruskal_helper]
+    set x := connected_component_of_unionFind_of_id uF e.node1 _ with h_x
+    set y := connected_component_of_unionFind_of_id uF e.node2 _ with h_y
+    simp [← h_x, ← h_y]
+    have h : [e] = [] ++ [e] := by
+      simp
+    by_cases h_eq : x = y
+    · simp [update_edgesSoFar, h_eq]
+      apply ih
+      · exact h_edgeList_not_con.right
+      · simp [update_unionFind]
+        exact h_uF_not_con
+    · simp [update_edgesSoFar, h_eq]
+      rw [h]
+      simp only [kruskal_helper.edgesSoFar_append]
+      simp
+      simp only [kruskal_helper.edgesSoFar_append] at ih
+      apply ih
+      · exact h_edgeList_not_con.right
+      · simp [update_unionFind, h_eq]
+        have h_x_ne_z : x ≠ z.id := by
+          simp at h_edgeList_not_con
+          simp [matching_edge] at h_matching_edge
+          rcases h_matching_edge.left.left with ⟨nx, h_nx_in, h_nx⟩
+          have h := (connected_component_of_unionFind_of_id_not_con h_z_in h_uF_not_con nx h_nx_in).mp
+          intro h_contra
+          simp [← h_contra, ← h_nx, h_x] at h
+          cases z
+          cases nx
+          simp at h
+          simp [h] at h_nx
+          simp [h_nx] at h_edgeList_not_con
+        have h_y_ne_z : y ≠ z.id := by
+          simp at h_edgeList_not_con
+          simp [matching_edge] at h_matching_edge
+          rcases h_matching_edge.left.right with ⟨ny, h_ny_in, h_ny⟩
+          have h := (connected_component_of_unionFind_of_id_not_con h_z_in h_uF_not_con ny h_ny_in).mp
+          intro h_contra
+          simp [← h_contra, ← h_ny, h_y] at h
+          cases z
+          cases ny
+          simp at h
+          simp [h] at h_ny
+          simp [h_ny] at h_edgeList_not_con
+        set uFLx := List.choose (fun a => a.nodeId = x ∧ a.ccId = x) uF.linkList _ with h_uFLx
+        set uFLy := List.choose (fun a => a.nodeId = y ∧ a.ccId = y) uF.linkList _ with h_uFLy
+        have h_uFLx_prop : uFLx.nodeId = x ∧ uFLx.ccId = x := List.choose_property (fun a => a.nodeId = x ∧ a.ccId = x) uF.linkList _
+        have h_uFLy_prop : uFLy.nodeId = y ∧ uFLy.ccId = y := List.choose_property (fun a => a.nodeId = y ∧ a.ccId = y) uF.linkList _
+        simp [← h_uFLx, ← h_uFLy]
+        -- by_cases h_rank_lt : uFLx.rank < uFLy.rank
+        -- · simp [h_rank_lt]
+        --   intro uFL h_uFL_in
+        --   rcases List.mem_or_eq_of_mem_set h_uFL_in with ⟨h_uFL_in⟩ | ⟨h_uFL_eq⟩
+        --   · rcases List.mem_or_eq_of_mem_set h_uFL_in with ⟨h_uFL_in⟩ | ⟨h_uFL_eq⟩
+        --     · exact h_uF_not_con uFL h_uFL_in
+        --     · simp [h_uFL_eq, h_uFLx_prop, h_uFLy_prop, h_x_ne_z, h_y_ne_z]
+        --   · simp [h_uFL_eq, h_uFLy_prop, h_y_ne_z]
+        by_cases h_rank_lt' : uFLy.rank < uFLx.rank
+        · simp [h_rank_lt']
+          intro uFL h_uFL_in
+          rcases List.mem_or_eq_of_mem_set h_uFL_in with ⟨h_uFL_in⟩ | ⟨h_uFL_eq⟩
+          · rcases List.mem_or_eq_of_mem_set h_uFL_in with ⟨h_uFL_in⟩ | ⟨h_uFL_eq⟩
+            · exact h_uF_not_con uFL h_uFL_in
+            · simp [h_uFL_eq, h_uFLx_prop, h_uFLy_prop, h_x_ne_z, h_y_ne_z]
+          · simp [h_uFL_eq, h_uFLx_prop, h_x_ne_z]
+        · simp [h_rank_lt']
+          intro uFL h_uFL_in
+          rcases List.mem_or_eq_of_mem_set h_uFL_in with ⟨h_uFL_in⟩ | ⟨h_uFL_eq⟩
+          · rcases List.mem_or_eq_of_mem_set h_uFL_in with ⟨h_uFL_in⟩ | ⟨h_uFL_eq⟩
+            · exact h_uF_not_con uFL h_uFL_in
+            · simp [h_uFL_eq, h_uFLx_prop, h_uFLy_prop, h_x_ne_z, h_y_ne_z]
+          · simp [h_uFL_eq, h_uFLy_prop, h_y_ne_z]
+
+theorem nodeList_of_kruskal_perm (edgeList : List edge) : List.Perm (nodeList_of_edgeList (kruskal_of_edgeList edgeList)) (nodeList_of_edgeList edgeList) := by
+  have h_nodup1 := nodeList_of_edgeList_nodup (kruskal_of_edgeList edgeList)
+  have h_nodup2 := nodeList_of_edgeList_nodup edgeList
+  apply (List.perm_ext_iff_of_nodup h_nodup1 h_nodup2).mpr
+  intro x
+  constructor
+  · intro h_x_in_nodeList_of_kruskal
+    simp [nodeList_of_edgeList] at h_x_in_nodeList_of_kruskal
+    have h_ex_e := (mem_nodeList_of_edgeList_helper_iff_node_in_edgeList (kruskal_of_edgeList edgeList) x).mp h_x_in_nodeList_of_kruskal
+    rcases h_ex_e with ⟨e, h_e_in_kruskal, h_e_con_x⟩
+    have h_e_in_edgeList := kruskal_sublist e h_e_in_kruskal
+    simp [nodeList_of_edgeList]
+    apply (mem_nodeList_of_edgeList_helper_iff_node_in_edgeList edgeList x).mpr
+    refine ⟨e, h_e_in_edgeList, h_e_con_x⟩
+  · intro h_x_in_nodeList_of_edgeList
+    simp [nodeList_of_edgeList] at h_x_in_nodeList_of_edgeList
+    have h_ex_e := (mem_nodeList_of_edgeList_helper_iff_node_in_edgeList edgeList x).mp h_x_in_nodeList_of_edgeList
+    rcases h_ex_e with ⟨e, h_e_in_kruskal, h_e_con_x⟩
+    simp [nodeList_of_edgeList]
+    simp [kruskal_of_edgeList, kruskal]
+    set edgeListSorted : List edge := edgeList.mergeSort with h_edgeListSorted
+    simp [← h_edgeListSorted]
+    have h_e_in_edgeListSorted : e ∈ edgeListSorted := by
+      simp [h_edgeListSorted, h_e_in_kruskal]
+    have h_ex : ∃ e_1 ∈ edgeListSorted, e_1.node1 = x.id ∨ e_1.node2 = x.id := by
+      refine ⟨e, h_e_in_edgeListSorted, h_e_con_x⟩
+    have h_split := prop_split (fun (e_1 : edge) => e_1.node1 = x.id ∨ e_1.node2 = x.id) h_ex
+    rcases h_split with ⟨l₁, l₂, f, h_split, h_f_con_x, h_l₁_not_con_x⟩
+    simp [h_split, nodeList_of_edgeList]
+    simp [nodeList_of_edgeList] at h_nodup2
+    set uF := init_unionFind (nodeList_of_edgeList_helper edgeList []) _
+    have h_edgeList_not_con : ∀ e ∈ l₁, ¬(e.node1 = x.id ∨ e.node2 = x.id) := by
+      exact h_l₁_not_con_x
+    have h_uF_not_con : ∀ uFL ∈ uF.linkList, uFL.ccId = x.id ↔ uFL.nodeId = x.id := by
+      have h_nonempty : nodeList_of_edgeList_helper edgeList [] ≠ [] := by
+        intro h_contra
+        simp [h_contra] at h_x_in_nodeList_of_edgeList
+      simp [uF, init_unionFind, h_nonempty, init_unionFind.linkList]
+      have h := init_unionFind.linkList.helper_all_self_connected (nodeList_of_edgeList_helper edgeList []) (nodeList_of_edgeList_helper edgeList []) (by simp [h_nonempty])
+      intro uFL h_uFL_in
+      simp [h uFL h_uFL_in]
+    have h_matching_edge : matching_edge (l₁ ++ f :: l₂) (nodeList_of_edgeList_helper edgeList []) := by
+      simp [← h_split, edgeListSorted, matching_edge]
+      intro g h_g_in
+      constructor
+      · have h := (mem_nodeList_of_edgeList_helper_iff_node_in_edgeList edgeList { id := g.node1 }).mpr
+        simp at h
+        have h := h g h_g_in
+        simp at h
+        refine ⟨{ id := g.node1 }, h, by simp⟩
+      · have h := (mem_nodeList_of_edgeList_helper_iff_node_in_edgeList edgeList { id := g.node2 }).mpr
+        simp at h
+        have h := h g h_g_in
+        simp at h
+        refine ⟨{ id := g.node2 }, h, by simp⟩
+    have h := kruskal_helper_not_con_invariant_append h_x_in_nodeList_of_edgeList h_edgeList_not_con h_uF_not_con (h_nodup := h_nodup2) (h_matching_edge := h_matching_edge) (edgesSoFar := []) (uF := uF) (edgeList₂ := f :: l₂)
+    rcases h with ⟨uF', h_eq, h_uF'_not_con⟩
+    simp [h_eq]
+    set k_l₁ := kruskal_helper l₁ (nodeList_of_edgeList_helper edgeList []) uF [] _ h_nodup2
+    simp [kruskal_helper]
+    have h_f_in : f ∈ edgeListSorted := by
+      simp [h_split]
+    simp [edgeListSorted] at h_f_in
+    have h_ex_f_node1 : ∃ x ∈ nodeList_of_edgeList_helper edgeList [], x.id = f.node1 := by
+      have h := (mem_nodeList_of_edgeList_helper_iff_node_in_edgeList edgeList { id := f.node1 }).mpr
+      simp at h
+      refine ⟨{ id := f.node1 }, ?_, by simp⟩
+      apply h f
+      · exact h_f_in
+      · simp
+    have h_ex_f_node2 : ∃ x ∈ nodeList_of_edgeList_helper edgeList [], x.id = f.node2 := by
+      have h := (mem_nodeList_of_edgeList_helper_iff_node_in_edgeList edgeList { id := f.node2 }).mpr
+      simp at h
+      refine ⟨{ id := f.node2 }, ?_, by simp⟩
+      apply h f
+      · exact h_f_in
+      · simp
+    have h_ne : connected_component_of_unionFind_of_id uF' f.node1 h_ex_f_node1 ≠ connected_component_of_unionFind_of_id uF' f.node2 h_ex_f_node2 := by
+      intro h_find_eq
+      have h := connected_component_of_unionFind_of_id_not_con h_x_in_nodeList_of_edgeList h_uF'_not_con
+      rcases h_f_con_x with h_f_con_x | h_f_con_x
+      · rcases h_ex_f_node2 with ⟨y, h_y_in, h_y⟩
+        have h_find_y := (h y h_y_in).mp
+        have h_find_x := (h x h_x_in_nodeList_of_edgeList).mpr
+        simp [← h_f_con_x] at h_find_x
+        simp [h_y, ← h_f_con_x, ← h_find_eq] at h_find_y
+        simp [h_find_x] at h_find_y
+        simp [h_find_y, ← h_f_con_x] at h_y
+        have h_contra := f.nodesLt
+        simp [h_y] at h_contra
+      · rcases h_ex_f_node1 with ⟨y, h_y_in, h_y⟩
+        have h_find_y := (h y h_y_in).mp
+        have h_find_x := (h x h_x_in_nodeList_of_edgeList).mpr
+        simp [← h_f_con_x] at h_find_x
+        simp [h_y, ← h_f_con_x, h_find_eq] at h_find_y
+        simp [h_find_x] at h_find_y
+        simp [h_find_y, ← h_f_con_x] at h_y
+        have h_contra := f.nodesLt
+        simp [h_y] at h_contra
+    simp [update_edgesSoFar, h_ne]
+    have h : f :: k_l₁ = [] ++ (f :: k_l₁) := by
+      simp
+    rw [h]
+    set uF'' := update_unionFind uF' (connected_component_of_unionFind_of_id uF' f.node1 _) (connected_component_of_unionFind_of_id uF' f.node2 _) _ _
+    rw [kruskal_helper.edgesSoFar_append (edgeList := l₂) (nodeList := nodeList_of_edgeList_helper edgeList []) (uF := uF'')]
+    apply (mem_nodeList_of_edgeList_helper_iff_node_in_edgeList (kruskal_helper l₂ (nodeList_of_edgeList_helper edgeList []) uF'' [] _ h_nodup2 ++ f :: k_l₁) x).mpr
+    refine ⟨f, ?_⟩
+    simp [h_f_con_x]
+
+theorem nodeList_of_edgeList_max_eq (edgeList : List edge) (h : edgeList ≠ []) : (nodeList_of_edgeList_max (kruskal_of_edgeList edgeList) (kruskal_nonempty edgeList h)).id.succ = (nodeList_of_edgeList_max edgeList h).id.succ := by
+  simp [nodeList_of_edgeList_max]
+  have h_edgeList_max := max_eq_maximum (nodeList_of_edgeList_nonempty edgeList h)
+  have h_kruskal_max := max_eq_maximum (nodeList_of_edgeList_nonempty (kruskal_of_edgeList edgeList) (kruskal_nonempty edgeList h))
+  have h_maximum_eq := List.Perm.maximum_eq (nodeList_of_kruskal_perm edgeList)
+  simp [h_maximum_eq, ← h_edgeList_max] at h_kruskal_max
+  simp [h_kruskal_max]
+
+theorem SimpleGraph_of_kruskal_IsSubgraph (edgeList : List edge) (h : edgeList ≠ []) : (SimpleGraph_of_kruskal edgeList h) ≤ (SimpleGraph_of_n_of_edgeList (nodeList_of_edgeList_max (kruskal_of_edgeList edgeList) _).id.succ edgeList h (nodeList_of_edgeList_max_eq edgeList h)) := by
+  simp [LE.le]
+  simp [SimpleGraph_of_kruskal, SimpleGraph_of_n_of_edgeList, SimpleGraph_of_edgeList]
+  intro u v e h_e_in h_adj
+  refine ⟨e, kruskal_sublist e h_e_in, h_adj⟩
+
+theorem connected_component_of_unionFind_of_id_of_update_unionFind_of_con
+  {nodeList : List node}
+  {uF : unionFind nodeList}
+  {a b c : Nat}
+  {h_a : ∃ x ∈ nodeList, x.id = a}
+  {h_b : ∃ x ∈ nodeList, x.id = b}
+  {h_c : ∃ x ∈ nodeList, x.id = c}
+  (h_con : connected_component_of_unionFind_of_id uF a h_a = connected_component_of_unionFind_of_id uF c h_c ∨ connected_component_of_unionFind_of_id uF b h_b = connected_component_of_unionFind_of_id uF c h_c)
+  : connected_component_of_unionFind_of_id (
+      update_unionFind uF
+        (connected_component_of_unionFind_of_id uF a h_a)
+        (connected_component_of_unionFind_of_id uF b h_b)
+        (exist_unionFindLink_of_connected_component_of_unionFind_of_id uF a h_a)
+        (exist_unionFindLink_of_connected_component_of_unionFind_of_id uF b h_b)
+    ) c h_c
+    = min (connected_component_of_unionFind_of_id uF a h_a) (connected_component_of_unionFind_of_id uF b h_b) := by
+  sorry
+
+theorem connected_component_of_unionFind_of_id_of_self
+  {nodeList : List node}
+  {uF : unionFind nodeList}
+  {id : Nat}
+  {h : ∃ x ∈ nodeList, x.id = id}
+  {h' : ∃ x ∈ nodeList, x.id = connected_component_of_unionFind_of_id uF id h}
+  : connected_component_of_unionFind_of_id uF (connected_component_of_unionFind_of_id uF id h) h' = connected_component_of_unionFind_of_id uF id h := by
+  set cc := connected_component_of_unionFind_of_id uF id h with ← h_cc
+  simp [h_cc]
+  have h_ex := exist_unionFindLink_of_connected_component_of_unionFind_of_id uF id h
+  simp [h_cc] at h_ex
+  rcases h_ex with ⟨uFLcc, h_uFLcc_self_con⟩
+  set uFLcc' := List.choose (fun x => x.nodeId = cc) uF.linkList (connected_component_of_unionFind_of_id._proof_1 uF cc (h_cc ▸ h') : ∃ x ∈ uF.linkList, x.nodeId = cc) with h_uFLcc'
+  have h_uFLcc'_prop := List.choose_property (fun x => x.nodeId = cc) uF.linkList (connected_component_of_unionFind_of_id._proof_1 uF cc (h_cc ▸ h') : ∃ x ∈ uF.linkList, x.nodeId = cc)
+  have h_uFLcc'_mem := List.choose_mem (fun x => x.nodeId = cc) uF.linkList (connected_component_of_unionFind_of_id._proof_1 uF cc (h_cc ▸ h') : ∃ x ∈ uF.linkList, x.nodeId = cc)
+  simp [connected_component_of_unionFind_of_id]
+  cases h' with
+  | intro x h_x =>
+  cases x
+  simp at h_x
+  simp [h_x.right] at h_x
+  have h_matching_nodeId := uF.matching_nodeId ⟨cc⟩ h_x
+  simp [ExistsUnique] at h_matching_nodeId
+  rcases h_matching_nodeId with ⟨uFLcc'', h_prop, h_unique⟩
+  simp [← h_uFLcc', h_unique uFLcc' h_uFLcc'_mem h_uFLcc'_prop.symm]
+  simp [← h_unique uFLcc h_uFLcc_self_con.left h_uFLcc_self_con.right.left.symm]
+  rw [connected_component_of_unionFind_of_unionFindLink]
+  simp [h_uFLcc_self_con]
+
+theorem node_of_uFL
+  {nodeList : List node}
+  {uF : unionFind nodeList}
+  {uFL : unionFindLink nodeList}
+  (h_in : uFL ∈ uF.linkList)
+  (h_nodup : nodeList.Nodup)
+  : ∃ x ∈ nodeList, x.id = uFL.nodeId := by
+  by_cases h_goal : ∃ x ∈ nodeList, x.id = uFL.nodeId
+  · exact h_goal
+  · simp at h_goal
+    have h_len := uF.matching_length
+    rcases mem_split h_in with ⟨l₁, l₂, h_split⟩
+    have h_matching_nodeId := uF.matching_nodeId
+    simp [h_split] at h_matching_nodeId
+    have h_matching_nodeId : ∀ x ∈ nodeList, ∃! y, (y ∈ l₁ ∨ y ∈ l₂) ∧ x.id = y.nodeId := by
+      intro x h_x_in
+      have h_matching_nodeId := h_matching_nodeId x h_x_in
+      have h_goal := h_goal x h_x_in
+      simp [ExistsUnique]
+      simp [ExistsUnique] at h_matching_nodeId
+      rcases h_matching_nodeId with ⟨y, h⟩
+      have h_y_ne_uFL : y ≠ uFL := by
+        intro h_eq
+        simp [← h_eq] at h_goal
+        simp [h_goal] at h
+      simp [h_y_ne_uFL] at h
+      refine ⟨y, ?_⟩
+      constructor
+      · simp [h]
+      · intro z h_z_in
+        have h' := h.right z
+        rcases h_z_in with h_z_in | h_z_in
+        · simp [h_z_in] at h'
+          exact h'
+        · simp [h_z_in] at h'
+          exact h'
+    induction nodeList with
+    | nil =>
+      simp at h_len
+      have h_nil := nil_of_length_zero h_len.symm
+      simp [h_nil] at h_in
+    | cons x l ih =>
+      have h_len' : uF.linkList.length = (l₁ ++ l₂).length + 1 := by
+        simp [h_split.left]
+        omega
+      simp [h_len'] at h_len
+      let f : node → unionFindLink (x :: l) := fun x_1 =>
+        if h_x_1_in : x_1 ∈ x :: l
+          then
+            have h_ex := h_matching_nodeId x_1 h_x_1_in
+            let uFL_1 : unionFindLink (x :: l) := by
+              simp [ExistsUnique] at h_ex
+              -- rcases h_ex with ⟨uFL_1, h⟩
+              exact Classical.choose h_ex
+            uFL_1
+          else
+            uFL
+      have h_f_id : ∀ a ∈ x :: l, (f a).nodeId = a.id := by
+        grind
+      have h_injectiv : ∀ a ∈ x :: l, ∀ b ∈ x :: l, f a = f b → a = b := by
+        intro a h_a_in b h_b_in h_f_eq
+        have h_id_eq : a.id = b.id := by
+          simp [← h_f_id a h_a_in, h_f_eq, h_f_id b h_b_in]
+        cases a
+        simp at h_id_eq
+        simp [h_id_eq]
+      have h_image : ∀ a ∈ x :: l, f a ∈ l₁ ++ l₂ := by
+        grind
+      have h := lenght_ge_of_injectiv h_nodup h_injectiv h_image
+      simp [h_len] at h
+
+theorem connected_component_of_unionFind_of_unionFindLink_of_self
+  {nodeList : List node}
+  {uF : unionFind nodeList}
+  {a b : unionFindLink nodeList}
+  {h_a_in : a ∈ uF.linkList}
+  {h_b_in : b ∈ uF.linkList}
+  (h_nodup : nodeList.Nodup)
+  : connected_component_of_unionFind_of_unionFindLink uF a h_a_in = connected_component_of_unionFind_of_unionFindLink uF b h_b_in →
+    connected_component_of_unionFind_of_id uF a.nodeId (node_of_uFL h_a_in h_nodup) =
+    connected_component_of_unionFind_of_id uF b.nodeId (node_of_uFL h_b_in h_nodup) := by
+  have h_unique_nodeId : ∀ uFL_1 ∈ uF.linkList, ∀ uFL_2 ∈ uF.linkList, uFL_1.nodeId = uFL_2.nodeId → uFL_1 = uFL_2 := by
+    intro uFL_1 h_uFL_1_in uFL_2 h_uFL_2_in h_nodeId_eq
+    have h_ex_node := node_of_uFL h_uFL_1_in h_nodup
+    rcases h_ex_node with ⟨x, h_x_in, h_x_id⟩
+    have h := uF.matching_nodeId x h_x_in
+    simp [ExistsUnique] at h
+    rcases h with ⟨uFL, h_uFL, h_unique⟩
+    have h_eq_1 := h_unique uFL_1 h_uFL_1_in h_x_id
+    have h_eq_2 := h_unique uFL_2 h_uFL_2_in (by simp [h_x_id, h_nodeId_eq])
+    simp [h_eq_1, h_eq_2]
+  rw [connected_component_of_unionFind_of_unionFindLink]
+  rw [connected_component_of_unionFind_of_unionFindLink]
+  simp [connected_component_of_unionFind_of_id]
+  have h_a'_prop := List.choose_property (fun x => x.nodeId = a.nodeId) uF.linkList (connected_component_of_unionFind_of_id._proof_1 uF a.nodeId (node_of_uFL h_a_in h_nodup) : ∃ x ∈ uF.linkList, x.nodeId = a.nodeId)
+  have h_a'_in := List.choose_mem (fun x => x.nodeId = a.nodeId) uF.linkList (connected_component_of_unionFind_of_id._proof_1 uF a.nodeId (node_of_uFL h_a_in h_nodup) : ∃ x ∈ uF.linkList, x.nodeId = a.nodeId)
+  set a' := List.choose (fun x => x.nodeId = a.nodeId) uF.linkList (connected_component_of_unionFind_of_id._proof_1 uF a.nodeId (node_of_uFL h_a_in h_nodup) : ∃ x ∈ uF.linkList, x.nodeId = a.nodeId) with ← h_a'
+  have h_b'_prop := List.choose_property (fun x => x.nodeId = b.nodeId) uF.linkList (connected_component_of_unionFind_of_id._proof_1 uF b.nodeId (node_of_uFL h_b_in h_nodup) : ∃ x ∈ uF.linkList, x.nodeId = b.nodeId)
+  have h_b'_in := List.choose_mem (fun x => x.nodeId = b.nodeId) uF.linkList (connected_component_of_unionFind_of_id._proof_1 uF b.nodeId (node_of_uFL h_b_in h_nodup) : ∃ x ∈ uF.linkList, x.nodeId = b.nodeId)
+  set b' := List.choose (fun x => x.nodeId = b.nodeId) uF.linkList (connected_component_of_unionFind_of_id._proof_1 uF b.nodeId (node_of_uFL h_b_in h_nodup) : ∃ x ∈ uF.linkList, x.nodeId = b.nodeId) with ← h_b'
+  simp [h_a', h_b', h_unique_nodeId a' h_a'_in a h_a_in (by simp [h_a'_prop]), h_unique_nodeId b' h_b'_in b h_b_in (by simp [h_b'_prop])]
+  split_ifs with h_a_self_con h_b_self_con
+  · intro h
+    rw [connected_component_of_unionFind_of_unionFindLink]
+    simp [← h_a_self_con, h_b_self_con, h]
+    rw [connected_component_of_unionFind_of_unionFindLink]
+    simp [h_b_self_con]
+  · intro h
+    rw [connected_component_of_unionFind_of_unionFindLink]
+    simp [← h_a_self_con]
+    rw [connected_component_of_unionFind_of_unionFindLink]
+    simp [h_b_self_con, h]
+  · intro h
+    rw [connected_component_of_unionFind_of_unionFindLink]
+    rw [connected_component_of_unionFind_of_unionFindLink]
+    rename_i h_b_self_con
+    simp [h_a_self_con, h_b_self_con, h]
+  · intro h
+    rw [connected_component_of_unionFind_of_unionFindLink]
+    rw [connected_component_of_unionFind_of_unionFindLink]
+    rename_i h_b_self_con
+    simp [h_a_self_con, h_b_self_con, h]
+
+def parent
+  {nodeList : List node}
+  {uF : unionFind nodeList}
+  (uFL : unionFindLink nodeList)
+  (h_in : uFL ∈ uF.linkList)
+  : unionFindLink nodeList
+  := List.choose (fun a => a.nodeId = uFL.ccId) uF.linkList (by rcases (uF.matching_ccId uFL h_in) with ⟨x, h, _⟩; rcases (uF.matching_nodeId x h.left) with ⟨uFL', h', _⟩; simp [← h.right]; refine ⟨uFL', by simp [h']⟩)
+
+def parent_path
+  {nodeList : List node}
+  (uF : unionFind nodeList)
+  (p : List (unionFindLink nodeList))
+  (h_in : ∀ a ∈ p, a ∈ uF.linkList)
+  : Prop :=
+  match p with
+  | [] => true
+  | a :: [] => true
+  | a :: b :: p' => b = parent (uF := uF) a (by grind) ∧ parent_path uF (b :: p') (by grind)
+
+theorem eq_cc
+  {nodeList : List node}
+  {uF : unionFind nodeList}
+  {uF' : unionFind nodeList}
+  {a b : unionFindLink nodeList}
+  {h_a_in : a ∈ uF.linkList}
+  {h_b_in : b ∈ uF'.linkList}
+  (h_eq : a = b)
+  (p : List (unionFindLink nodeList))
+  (h_path_in : ∀ a ∈ p, a ∈ uF.linkList)
+  (h_path_in' : ∀ a ∈ p, a ∈ uF'.linkList)
+  (h_path : parent_path uF p h_path_in)
+  (h_path' : parent_path uF' p h_path_in')
+  (h_path_start : ∃ p', p = a :: p')
+  (h_path_end : ∃ c ∈ p, c.nodeId = c.ccId)
+  -- parent_path a = parent_path b
+  : connected_component_of_unionFind_of_unionFindLink uF a h_a_in = connected_component_of_unionFind_of_unionFindLink uF' b h_b_in := by
+  induction a, h_a_in using connected_component_of_unionFind_of_unionFindLink.induct generalizing b p with
+  | case1 x h_x_in h_x_self_con =>
+    rw [connected_component_of_unionFind_of_unionFindLink]
+    simp [h_x_self_con, ← h_eq]
+    rw [connected_component_of_unionFind_of_unionFindLink]
+    simp [h_x_self_con]
+  | case2 x h_x_in h_x_not_self_con y h_y_in h_rank_lt =>
+    rename_i ih
+    simp [← h_eq]
+    rw [connected_component_of_unionFind_of_unionFindLink]
+    rw [connected_component_of_unionFind_of_unionFindLink]
+    simp [h_x_not_self_con]
+    have h_y_eq_parent : y = parent x h_x_in := by
+      simp [y, parent]
+    rcases h_path_start with ⟨p', h_path_start⟩
+    cases p' with
+    | nil =>
+      simp [h_path_start] at h_path_end
+      simp [h_path_end] at h_x_not_self_con
+    | cons z p' =>
+      have h_z_eq_y : z = y := by
+        simp [h_path_start, parent_path] at h_path
+        simp [h_path, h_y_eq_parent]
+      simp [h_z_eq_y] at h_path_start
+      have h_y_eq_parent' : y = parent b h_b_in := by
+        simp [h_path_start, parent_path, h_eq] at h_path'
+        simp [← h_path'.left]
+      have h_y : List.choose (fun y => y.nodeId = x.ccId) uF.linkList (connected_component_of_unionFind_of_unionFindLink._unary._proof_1 uF x h_x_in : ∃ y ∈ uF.linkList, y.nodeId = x.ccId) = y := by
+        simp [y]
+      simp [parent, ← h_eq] at h_y_eq_parent'
+      simp [h_y, ← h_y_eq_parent']
+      apply ih (by rfl) (y :: p')
+      · simp [h_path_start, parent_path] at h_path
+        simp [h_path.right]
+      · simp [h_path_start, parent_path] at h_path'
+        simp [h_path'.right]
+      · refine ⟨p', rfl⟩
+      · simp [h_path_start, ne_comm.mp h_x_not_self_con] at h_path_end
+        simp [h_path_end]
+      · simp [h_path_start] at h_path_in
+        simp
+        exact h_path_in.right
+      · simp [h_path_start] at h_path_in'
+        simp
+        exact h_path_in'.right
+
+def get_parent_path
+  {nodeList : List node}
+  {uF : unionFind nodeList}
+  {uFL : unionFindLink nodeList}
+  (h_in : uFL ∈ uF.linkList)
+  : List (unionFindLink nodeList) :=
+  if h_self_con : uFL.nodeId = uFL.ccId
+    then
+      (uFL :: [])
+    else
+      (uFL :: (get_parent_path (uFL := parent uFL h_in) (by simp [parent, List.choose_mem]) (uF := uF)))
+termination_by nodeList.length - uFL.rank
+  decreasing_by
+  have h_lt := uFL.rank.isLt
+  have h_increase : uFL.rank.val < (parent uFL h_in).rank.val := by
+    have h := uF.matching_rank uFL h_in
+    simp [h_self_con] at h
+    simp [parent, h]
+  exact Nat.sub_lt_sub_left h_lt h_increase
+
+theorem get_parent_path_in
+  {nodeList : List node}
+  {uF : unionFind nodeList}
+  {uFL : unionFindLink nodeList}
+  (h_in : uFL ∈ uF.linkList)
+  : ∀ a ∈ (get_parent_path h_in), a ∈ uF.linkList := by
+  fun_induction get_parent_path with
+  | case1 uFL h_in _ =>
+    simp [h_in]
+  | case2 uFL h_in _ ih =>
+    simp [h_in]
+    exact ih
+
+theorem get_parent_path_is_parent_path
+  {nodeList : List node}
+  {uF : unionFind nodeList}
+  {uFL : unionFindLink nodeList}
+  (h_in : uFL ∈ uF.linkList)
+  : parent_path uF (get_parent_path h_in) (get_parent_path_in h_in) := by
+  fun_induction get_parent_path with
+  | case1 uFL h_in h_self_con =>
+    unfold get_parent_path
+    simp [h_self_con, parent_path]
+  | case2 uFL h_in h_not_self_con ih =>
+    unfold get_parent_path
+    simp [h_not_self_con]
+    unfold get_parent_path
+    unfold get_parent_path at ih
+    split_ifs with h_self_con
+    · simp [parent_path]
+    · simp [parent_path]
+      simp [h_self_con] at ih
+      exact ih
+
+theorem get_parent_path_start
+  {nodeList : List node}
+  {uF : unionFind nodeList}
+  {uFL : unionFindLink nodeList}
+  (h_in : uFL ∈ uF.linkList)
+  : ∃ p', (get_parent_path h_in) = uFL :: p' := by
+  unfold get_parent_path
+  split_ifs
+  · simp
+  · simp
+
+theorem get_parent_path_end
+  {nodeList : List node}
+  {uF : unionFind nodeList}
+  {uFL : unionFindLink nodeList}
+  (h_in : uFL ∈ uF.linkList)
+  : ∃ a ∈ (get_parent_path h_in), a.nodeId = a.ccId := by
+  fun_induction get_parent_path with
+  | case1 uFL h_in h_self_con =>
+    simp [h_self_con]
+  | case2 uFL h_in h_not_self_con ih =>
+    simp [h_not_self_con]
+    exact ih
+
+theorem connected_component_of_unionFind_of_id_of_update_unionFind_of_not_con
+  {nodeList : List node}
+  {uF : unionFind nodeList}
+  {a b c : Nat}
+  {h_a : ∃ x ∈ nodeList, x.id = a}
+  {h_b : ∃ x ∈ nodeList, x.id = b}
+  {h_c : ∃ x ∈ nodeList, x.id = c}
+  (h_not_con : ¬(connected_component_of_unionFind_of_id uF a h_a = connected_component_of_unionFind_of_id uF c h_c ∨ connected_component_of_unionFind_of_id uF b h_b = connected_component_of_unionFind_of_id uF c h_c))
+  : connected_component_of_unionFind_of_id (
+      update_unionFind uF
+        (connected_component_of_unionFind_of_id uF a h_a)
+        (connected_component_of_unionFind_of_id uF b h_b)
+        (exist_unionFindLink_of_connected_component_of_unionFind_of_id uF a h_a)
+        (exist_unionFindLink_of_connected_component_of_unionFind_of_id uF b h_b)
+    ) c h_c
+    = connected_component_of_unionFind_of_id uF c h_c := by
+  simp at h_not_con
+  set updated_uF := update_unionFind uF (connected_component_of_unionFind_of_id uF a h_a) (connected_component_of_unionFind_of_id uF b h_b) (exist_unionFindLink_of_connected_component_of_unionFind_of_id uF a h_a) (exist_unionFindLink_of_connected_component_of_unionFind_of_id uF b h_b) with h_updated_uF
+  set cca := connected_component_of_unionFind_of_id uF a h_a with h_cca
+  set ccb := connected_component_of_unionFind_of_id uF b h_b with h_ccb
+  set ccc := connected_component_of_unionFind_of_id uF c h_c with h_ccc
+  set uFLa := List.choose (fun a => a.nodeId = cca ∧ a.ccId = cca) uF.linkList (Eq.ndrec (motive := fun p => ∀ [DecidablePred p], ∃ a ∈ uF.linkList, p a) (fun [DecidablePred fun a_1 => a_1.nodeId = connected_component_of_unionFind_of_id uF a h_a ∧ a_1.ccId = connected_component_of_unionFind_of_id uF a h_a] => Eq.refl uF.linkList ▸ exist_unionFindLink_of_connected_component_of_unionFind_of_id uF a h_a) (funext fun a_1 => congr (congrArg And (congrArg (Eq a_1.nodeId) (Eq.symm h_cca))) (congrArg (Eq a_1.ccId) (Eq.symm h_cca))) : ∃ a ∈ uF.linkList, (fun a => a.nodeId = cca ∧ a.ccId = cca) a) with h_uFLa
+  set uFLb := List.choose (fun a => a.nodeId = ccb ∧ a.ccId = ccb) uF.linkList (Eq.ndrec (motive := fun p => ∀ [DecidablePred p], ∃ a ∈ uF.linkList, p a) (fun [DecidablePred fun a_1 => a_1.nodeId = connected_component_of_unionFind_of_id uF b h_b ∧ a_1.ccId = connected_component_of_unionFind_of_id uF b h_b] => Eq.refl uF.linkList ▸ exist_unionFindLink_of_connected_component_of_unionFind_of_id uF b h_b) (funext fun a_1 => congr (congrArg And (congrArg (Eq a_1.nodeId) (Eq.symm h_ccb))) (congrArg (Eq a_1.ccId) (Eq.symm h_ccb))) : ∃ a ∈ uF.linkList, (fun a => a.nodeId = ccb ∧ a.ccId = ccb) a) with h_uFLb
+  simp [← h_cca, ← h_ccb, update_unionFind, ← h_uFLa, ← h_uFLb, h_updated_uF]
+  have h_c_ne_a : c ≠ a := by
+    intro h_eq
+    simp [cca, ccc, h_eq] at h_not_con
+  have h_c_ne_b : c ≠ b := by
+    intro h_eq
+    simp [ccb, ccc, h_eq] at h_not_con
+  have h_c_ne_cca : c ≠ cca := by
+    intro h_eq
+    have h := h_not_con.left
+    simp [ccc, h_eq, cca, connected_component_of_unionFind_of_id_of_self] at h
+  have h_c_ne_ccb : c ≠ ccb := by
+    intro h_eq
+    have h := h_not_con.right
+    simp [ccc, h_eq, ccb, connected_component_of_unionFind_of_id_of_self] at h
+  have h_not_con' : ¬(connected_component_of_unionFind_of_id updated_uF a h_a = connected_component_of_unionFind_of_id updated_uF c h_c ∨ connected_component_of_unionFind_of_id updated_uF b h_b = connected_component_of_unionFind_of_id updated_uF c h_c) := by
+    sorry
+  split_ifs with h_eq h_rank_lt'
+  · rfl
+  -- wegen h_rank_lt kürzung
+  -- · set uFLa' : unionFindLink nodeList := { nodeId := uFLa.nodeId, ccId := uFLb.ccId, rank := uFLa.rank } with h_uFLa'
+  --   set uFLb' : unionFindLink nodeList := { nodeId := uFLb.nodeId, ccId := uFLb.ccId, rank := ⟨max (↑uFLb.rank) (↑uFLa.rank + 1), sorry⟩ } with h_uFLb'
+  --   simp [← h_uFLa', ← h_uFLb']
+  --   simp [connected_component_of_unionFind_of_id]
+  --   have h_uFLc_prop := List.choose_property (fun a => a.nodeId = c) ((uF.linkList.set (List.idxOf uFLa uF.linkList) uFLa').set (List.idxOf uFLb uF.linkList) uFLb') sorry
+  --   have h_uFLc_mem := List.choose_mem (fun a => a.nodeId = c) ((uF.linkList.set (List.idxOf uFLa uF.linkList) uFLa').set (List.idxOf uFLb uF.linkList) uFLb') sorry
+  --   set uFLc := List.choose (fun a => a.nodeId = c) ((uF.linkList.set (List.idxOf uFLa uF.linkList) uFLa').set (List.idxOf uFLb uF.linkList) uFLb') sorry with h_uFLc
+  --   simp [← h_uFLc]
+  --   simp [choose_findIdx] at h_uFLc
+  --   simp [findIdx_set_of_not_prop sorry sorry sorry] at h_uFLc
+  --   have h_idx_ne_b : List.idxOf uFLb uF.linkList ≠ List.findIdx (fun b => decide (b.nodeId = c)) uF.linkList := by sorry
+  --   have h_idx_ne_a : List.idxOf uFLa uF.linkList ≠ List.findIdx (fun b => decide (b.nodeId = c)) uF.linkList := by sorry
+  --   simp [getElem_set_of_ne_index sorry h_idx_ne_b (j := List.findIdx (fun b => decide (b.nodeId = c)) uF.linkList)] at h_uFLc
+  --   simp [getElem_set_of_ne_index sorry h_idx_ne_a (j := List.findIdx (fun b => decide (b.nodeId = c)) uF.linkList)] at h_uFLc
+  --   have h_choose : uF.linkList[List.findIdx (fun b => decide (b.nodeId = c)) uF.linkList]'sorry = List.choose (fun x => x.nodeId = c) uF.linkList sorry := by
+  --     simp [choose_findIdx]
+  --   simp [h_choose] at h_uFLc
+  --   by_cases h_self_con : uFLc.nodeId = uFLc.ccId
+  --   · simp [ccc, connected_component_of_unionFind_of_id]
+  --     rw [connected_component_of_unionFind_of_unionFindLink]
+  --     rw [connected_component_of_unionFind_of_unionFindLink]
+  --     simp [← h_uFLc, h_self_con]
+  --   · simp [ccc, connected_component_of_unionFind_of_id]
+  --     simp [← h_uFLc]
+  --     simp [update_unionFind, ← h_cca, ← h_ccb, ← h_uFLa, ← h_uFLb, ← h_uFLa', ← h_uFLb'] at h_updated_uF
+  --     simp [h_eq, h_rank_lt] at h_updated_uF
+  --     simp [← h_updated_uF]
+  --     -- nächster Schritt
+  --     -- connected_component_of_unionFind_of_id updated_uF a h_a = connected_component_of_unionFind_of_id updated_uF c h_c
+  --     -- connected_component_of_unionFind_of_id updated_uF b h_b = connected_component_of_unionFind_of_id updated_uF c h_c
+  --     have h_uFLc_in : uFLc ∈ uF.linkList := by
+  --       simp [h_uFLc, List.choose_mem]
+  --     have h_uFLc_in' : uFLc ∈ updated_uF.linkList := by
+  --       simp [h_rank_lt] at h_uFLb'
+  --       simp [updated_uF, update_unionFind, ← h_cca, ← h_ccb, h_eq, ← h_uFLa, ← h_uFLb, h_rank_lt, ← h_uFLa', ← h_uFLb', h_uFLc_mem]
+  --     set p : List (unionFindLink nodeList) := get_parent_path h_uFLc_in with ← h_p
+  --     let p' : List (unionFindLink nodeList) := get_parent_path h_uFLc_in'
+  --     have h_p_start := get_parent_path_start h_uFLc_in
+  --     -- simp [h_p] at h_p_start
+  --     have h_p_eq_p' : p = p' := by
+  --       sorry
+  --     apply eq_cc rfl p
+  --     · simp [h_p_eq_p', p'] -- kann ich diese beiden auch für p zeigen?
+  --       exact get_parent_path_is_parent_path h_uFLc_in'
+  --     · simp [p]
+  --       exact get_parent_path_is_parent_path h_uFLc_in
+  --     · simp [p]
+  --       exact get_parent_path_start h_uFLc_in
+  --     · simp [p]
+  --       exact get_parent_path_end h_uFLc_in
+  --     · simp [p]
+  --       have h_path :
+  --         ∀ (z : unionFindLink nodeList)
+  --           (h_z_in : z ∈ uF.linkList)
+  --           (h_z_in' : z ∈ updated_uF.linkList)
+  --           (h_not : ¬(connected_component_of_unionFind_of_id updated_uF a h_a = connected_component_of_unionFind_of_unionFindLink updated_uF z h_z_in' ∨ connected_component_of_unionFind_of_id updated_uF b h_b = connected_component_of_unionFind_of_unionFindLink updated_uF z h_z_in')),
+  --           ∀ a ∈ get_parent_path h_z_in,
+  --             a ∈ updated_uF.linkList := by
+  --         intro z h_z_in
+  --         induction z, h_z_in using get_parent_path.induct with
+  --         | case1 =>
+  --           sorry
+  --         | case2 =>
+  --           sorry
+  --       have h_ccc'_eq : connected_component_of_unionFind_of_id updated_uF c h_c = connected_component_of_unionFind_of_unionFindLink updated_uF uFLc h_uFLc_in' := by sorry
+  --       simp only [h_ccc'_eq] at h_not_con'
+  --       exact h_path uFLc h_uFLc_in h_uFLc_in' h_not_con'
+  --     -- · simp [h_p_eq_p', p'] -- kann ich diese beiden auch für p zeigen?
+  --     --   exact get_parent_path_in h_uFLc_in'
+  · sorry
+  · sorry
+
+abbrev _root_.SimpleGraph.Walk.start {a b : α} {G : SimpleGraph α} (_ : G.Walk a b) : α := a
+
+def walk_of_subgraph [DecidableEq α] (G H : SimpleGraph α) (h_sub : G ≤ H) (a b : α) (p : G.Walk a b) : H.Walk a b :=
+  match h_p : p with
+  | .nil =>
+    SimpleGraph.Walk.nil
+  | .cons h_adj p' =>
+    let c := p'.start
+    have h_adj' : H.Adj a c := by
+      simp [LE.le] at h_sub
+      apply h_sub
+      exact h_adj
+    SimpleGraph.Walk.cons h_adj' (walk_of_subgraph G H h_sub c b p')
+termination_by p.length
+  decreasing_by
+  simp
+
+theorem not_reachable_of_neighbor_not_reachable (G : SimpleGraph α) (a b c : α) (h_adj : G.Adj a b) (h_not_reachable : ¬G.Reachable a c) : ¬G.Reachable b c := by
+  intro h_reachable
+  simp [SimpleGraph.Reachable] at h_reachable h_not_reachable
+  cases h_reachable with
+  | intro p =>
+  let q : G.Walk a c := SimpleGraph.Walk.cons h_adj p
+  cases h_not_reachable with
+  | mk h_not_reachable =>
+  have h_contra := h_not_reachable q
+  contradiction
+
+def walk_of_keine_ahnung
+  (G H : SimpleGraph (Fin n))
+  (a b : (Fin n))
+  (p : G.Walk a b)
+  (edgesSoFar : List edge)
+  (e : edge)
+  (h_G : G.Adj = fun (a b : Fin n) => (e.node1 = ↑a ∧ e.node2 = ↑b ∨ e.node1 = ↑b ∧ e.node2 = ↑a) ∨ ∃ f ∈ edgesSoFar, f.node1 = ↑a ∧ f.node2 = ↑b ∨ f.node1 = ↑b ∧ f.node2 = ↑a)
+  (h_H : H.Adj = fun (a b : Fin n) => ∃ f ∈ edgesSoFar, f.node1 = ↑a ∧ f.node2 = ↑b ∨ f.node1 = ↑b ∧ f.node2 = ↑a)
+  {h_lt₁ : e.node1 < n}
+  {h_lt₂ : e.node2 < n}
+  (h_not_reachable1 : ¬H.Reachable a ⟨e.node1, h_lt₁⟩)
+  (h_not_reachable2 : ¬H.Reachable a ⟨e.node2, h_lt₂⟩)
+  : H.Walk a b :=
+  match h_p : p with
+  | .nil =>
+    SimpleGraph.Walk.nil
+  | .cons h_adj p' =>
+    let c := p'.start
+    have h_adj' : H.Adj a c := by
+      have h_e1_ne_a : e.node1 ≠ a.val := by
+        intro h_eq
+        simp [h_eq] at h_not_reachable1
+      have h_e2_ne_a : e.node2 ≠ a.val := by
+        intro h_eq
+        simp [h_eq] at h_not_reachable2
+      simp [h_G, h_e1_ne_a, h_e2_ne_a] at h_adj
+      simp [h_H, h_adj, c]
+    have h_not_reachable_c_e1 := not_reachable_of_neighbor_not_reachable H a c ⟨e.node1, h_lt₁⟩ h_adj' h_not_reachable1
+    have h_not_reachable_c_e2 := not_reachable_of_neighbor_not_reachable H a c ⟨e.node2, h_lt₂⟩ h_adj' h_not_reachable2
+    SimpleGraph.Walk.cons h_adj' (walk_of_keine_ahnung G H c b p' edgesSoFar e h_G h_H h_not_reachable_c_e1 h_not_reachable_c_e2)
+termination_by p.length
+  decreasing_by
+  simp
+
+theorem kruskal_helper_Reachable_iff_con
+  {edgeList : List edge}
+  {e : edge}
+  {nodeList : List node}
+  {uF : unionFind nodeList}
+  {edgesSoFar : List edge}
+  {h_matching_edge : matching_edge edgeList nodeList}
+  {h_nodup : nodeList.Nodup}
+  (h_nonempty : nodeList ≠ [])
+  (h_ex1 : ∃ x ∈ nodeList, x.id = e.node1)
+  (h_ex2 : ∃ x ∈ nodeList, x.id = e.node2)
+  (h_e1_self_con : ∃ uFL ∈ uF.linkList, uFL.nodeId = connected_component_of_unionFind_of_id uF e.node1 h_ex1 ∧ uFL.ccId = connected_component_of_unionFind_of_id uF e.node1 h_ex1)
+  (h_e2_self_con : ∃ uFL ∈ uF.linkList, uFL.nodeId = connected_component_of_unionFind_of_id uF e.node2 h_ex2 ∧ uFL.ccId = connected_component_of_unionFind_of_id uF e.node2 h_ex2)
+  -- {h_symm : Symmetric fun (a b : Fin (nodeList.max h_nonempty).id.succ) => ∃ e ∈ kruskal_helper edgeList nodeList uF edgesSoFar h_matching_edge h_nodup, e.node1 = ↑a ∧ e.node2 = ↑b ∨ e.node1 = ↑b ∧ e.node2 = ↑a}
+  -- {h_loopless : Std.Irrefl fun (a b : Fin (nodeList.max h_nonempty).id.succ) => ∃ e ∈ kruskal_helper edgeList nodeList uF edgesSoFar h_matching_edge h_nodup, e.node1 = ↑a ∧ e.node2 = ↑b ∨ e.node1 = ↑b ∧ e.node2 = ↑a}
+  (h_invariant : (fun (G : SimpleGraph (Fin (nodeList.max h_nonempty).id.succ)) => ∀ (a b : Fin _), (h_ex_x : ∃ x ∈ nodeList, x.id = ↑a) → (h_ex_y : ∃ x ∈ nodeList, x.id = ↑b) → (G.Reachable a b ↔ connected_component_of_unionFind_of_id uF a.val h_ex_x = connected_component_of_unionFind_of_id uF b.val h_ex_y)) { Adj := fun a b => ∃ f ∈ edgesSoFar, f.node1 = ↑a ∧ f.node2 = ↑b ∨ f.node1 = ↑b ∧ f.node2 = ↑a, symm := (by simp [Symmetric]; intro a b e; grind), loopless := (by simp [irrefl_def]; intro a e _ h_eq₁ h_eq₂; have h_lt := e.nodesLt; simp [h_eq₁, h_eq₂] at h_lt)})
+  : (fun
+      (G : SimpleGraph (Fin (nodeList.max h_nonempty).id.succ)) => ∀ (a b : Fin _), (h_ex_x : ∃ x ∈ nodeList, x.id = ↑a) →
+      (h_ex_y : ∃ x ∈ nodeList, x.id = ↑b) →
+      (G.Reachable a b ↔
+        connected_component_of_unionFind_of_id (update_unionFind uF (connected_component_of_unionFind_of_id uF e.node1 h_ex1) (connected_component_of_unionFind_of_id uF e.node2 h_ex2) h_e1_self_con h_e2_self_con) a.val h_ex_x =
+        connected_component_of_unionFind_of_id (update_unionFind uF (connected_component_of_unionFind_of_id uF e.node1 h_ex1) (connected_component_of_unionFind_of_id uF e.node2 h_ex2) h_e1_self_con h_e2_self_con) b.val h_ex_y))
+    { Adj := fun a b => ∃ f ∈ update_edgesSoFar edgesSoFar e (connected_component_of_unionFind_of_id uF e.node1 h_ex1) (connected_component_of_unionFind_of_id uF e.node2 h_ex2), f.node1 = ↑a ∧ f.node2 = ↑b ∨ f.node1 = ↑b ∧ f.node2 = ↑a, symm := (by simp [Symmetric]; intro a b e; grind), loopless := (by simp [irrefl_def]; intro a e _ h_eq₁ h_eq₂; have h_lt := e.nodesLt; simp [h_eq₁, h_eq₂] at h_lt) } := by
+  simp
+  intro a b x h_x_in h_x y h_y_in h_y
+  set cce1 := connected_component_of_unionFind_of_id uF e.node1 h_ex1 with ← h_cce1
+  set cce2 := connected_component_of_unionFind_of_id uF e.node2 h_ex2 with ← h_cce2
+  set cca := connected_component_of_unionFind_of_id uF ↑a ⟨x, h_x_in, h_x⟩ with h_cca
+  set ccb := connected_component_of_unionFind_of_id uF ↑b ⟨y, h_y_in, h_y⟩ with h_ccb
+  simp [h_cce1, h_cce2]
+  by_cases h_cc_eq : cce1 = cce2
+  · simp [update_edgesSoFar, update_unionFind, h_cc_eq]
+    simp at h_invariant
+    exact h_invariant a b x h_x_in h_x y h_y_in h_y
+  · simp [update_edgesSoFar, h_cc_eq] -- , update_unionFind
+    set G :  SimpleGraph (Fin (nodeList.max h_nonempty).id.succ) := { Adj := fun a b => ∃ f ∈ edgesSoFar, f.node1 = ↑a ∧ f.node2 = ↑b ∨ f.node1 = ↑b ∧ f.node2 = ↑a, symm := (by simp [Symmetric]; intro a b e; grind), loopless := (by simp [irrefl_def]; intro a e _ h_eq₁ h_eq₂; have h_lt := e.nodesLt; simp [h_eq₁, h_eq₂] at h_lt) }
+    set H :  SimpleGraph (Fin (nodeList.max h_nonempty).id.succ) := { Adj := fun a b => (e.node1 = ↑a ∧ e.node2 = ↑b ∨ e.node1 = ↑b ∧ e.node2 = ↑a) ∨ ∃ f ∈ edgesSoFar, f.node1 = ↑a ∧ f.node2 = ↑b ∨ f.node1 = ↑b ∧ f.node2 = ↑a, symm := (by simp [Symmetric]; intro a b e; grind), loopless :=  (by simp [irrefl_def]; intro a; constructor; grind; intro e _ h_eq₁ h_eq₂; have h_lt := e.nodesLt; simp [h_eq₁, h_eq₂] at h_lt) }
+    have h_subgraph : G ≤ H := by
+      simp [LE.le, G, H]
+      intro u v e h_e_in h_e_con
+      right
+      refine ⟨e, h_e_in, h_e_con⟩
+    rcases h_ex1 with ⟨e1, h_e1_in, h_e1⟩
+    cases e1
+    simp at h_e1
+    simp [h_e1] at h_e1_in
+    rcases h_ex2 with ⟨e2, h_e2_in, h_e2⟩
+    cases e2
+    simp at h_e2
+    simp [h_e2] at h_e2_in
+    have h_e1_lt_max : e.node1 < (nodeList.max h_nonempty).id + 1 := by
+      simp
+      have h_e1_lt_max : { id := e.node1 } ≤ nodeList.max h_nonempty := by
+        simp [List.le_max_of_mem h_e1_in]
+      exact h_e1_lt_max
+    have h_e2_lt_max : e.node2 < (nodeList.max h_nonempty).id + 1 := by
+      simp
+      have h_e2_lt_max : { id := e.node2 } ≤ nodeList.max h_nonempty := by
+        simp [List.le_max_of_mem h_e2_in]
+      exact h_e2_lt_max
+    by_cases h_con : cce1 = cca ∧ cce2 = ccb ∨ cce1 = ccb ∧ cce2 = cca
+    · by_cases h_con' : cce1 = cca ∧ cce2 = ccb
+      · simp [h_con']
+        have h_cc_ne : cca ≠ ccb := by
+          simp [h_con'] at h_cc_eq
+          exact h_cc_eq
+        have h_a_ne_b : a ≠ b := by
+          intro h
+          simp [h, cca, ccb] at h_cc_ne
+        simp [update_unionFind, h_cc_ne]
+        simp [h_con'] at h_e1_self_con h_e2_self_con
+        set choosea := List.choose (fun a => a.nodeId = cca ∧ a.ccId = cca) uF.linkList h_e1_self_con with ← h_choosea
+        set chooseb := List.choose (fun a => a.nodeId = ccb ∧ a.ccId = ccb) uF.linkList h_e2_self_con with ← h_chooseb
+        simp [h_choosea, h_chooseb]
+        split_ifs with h_rank_lt'
+        -- wegen h_rank_lt kürzung
+        -- · constructor
+        --   · intro h_reachable
+        --     -- für beide seiten zeigen, dass es auf ccb hinaus läuft
+        --     have h_left_ccb : connected_component_of_unionFind_of_id (update_unionFind uF cca ccb (h_con'.1 ▸ h_e1_self_con) (h_con'.2 ▸ h_e2_self_con)) ↑a (Exists.intro x ⟨h_x_in, h_x⟩) = ccb := by
+        --       sorry
+        --     have h_right_ccb : connected_component_of_unionFind_of_id (update_unionFind uF cca ccb (h_con'.1 ▸ h_e1_self_con) (h_con'.2 ▸ h_e2_self_con)) ↑b (Exists.intro y ⟨h_y_in, h_y⟩) = ccb := by
+        --       sorry
+        --     simp [update_unionFind, h_cc_ne, h_choosea, h_chooseb, h_rank_lt] at h_left_ccb h_right_ccb
+        --     simp [h_rank_lt, h_left_ccb, h_right_ccb]
+        --   · intro h_cc_eq'
+        --     simp [SimpleGraph.Reachable]
+        --     have h_p1 := (h_invariant a ⟨e.node1, h_e1_lt_max⟩ ⟨x, h_x_in, h_x⟩ ⟨{ id := e.node1 }, h_e1_in, by simp⟩).mpr (by simp [cca, cce1] at h_con'; simp [h_con'])
+        --     have h_p2 := (h_invariant ⟨e.node2, h_e2_lt_max⟩ b ⟨{ id := e.node2 }, h_e2_in, by simp⟩ ⟨y, h_y_in, h_y⟩).mpr (by simp [ccb, cce2] at h_con'; simp [h_con'])
+        --     simp [SimpleGraph.Reachable] at h_p1 h_p2
+        --     cases h_p1 with
+        --     | intro p1 =>
+        --     cases h_p2 with
+        --     | intro p2 =>
+        --     let q1 : H.Walk a ⟨e.node1, h_e1_lt_max⟩ := walk_of_subgraph G H h_subgraph a ⟨e.node1, h_e1_lt_max⟩ p1
+        --     let q2 : H.Walk ⟨e.node2, h_e2_lt_max⟩ b := walk_of_subgraph G H h_subgraph ⟨e.node2, h_e2_lt_max⟩ b p2
+        --     let q2' : H.Walk ⟨e.node1, h_e1_lt_max⟩ b := SimpleGraph.Walk.cons (by simp [H]) q2
+        --     let q : H.Walk a b := SimpleGraph.Walk.append q1 q2'
+        --     exact ⟨q⟩
+        · sorry -- basicliy coppy paste
+        · sorry -- basicliy coppy paste
+      · simp [h_con'] at h_con
+        simp [h_con]
+        sorry -- basicliy coppy paste (incusive split_ifs)
+    · have h_a_not_con : ¬(cce1 = cca ∨ cce2 = cca) := by -- falsch bzw. deckt nicht alle fälle ab
+        sorry
+      have h_b_not_con : ¬(cce1 = ccb ∨ cce2 = ccb) := by -- falsch bzw. deckt nicht alle fälle ab
+        sorry
+      simp only [cce1, cce2, cca] at h_a_not_con
+      simp only [cce1, cce2, ccb] at h_b_not_con
+      simp only [cce1, cce2]
+      simp [connected_component_of_unionFind_of_id_of_update_unionFind_of_not_con h_a_not_con, connected_component_of_unionFind_of_id_of_update_unionFind_of_not_con h_b_not_con]
+      simp at h_invariant
+      constructor
+      · intro h_reachable
+        apply (h_invariant a b x h_x_in h_x y h_y_in h_y).mp
+        simp [Reachable] at h_reachable
+        simp [Reachable]
+        cases h_reachable with
+        | intro p =>
+        -- set G :  SimpleGraph (Fin (nodeList.max h_nonempty).id.succ) := { Adj := fun a b => ∃ f ∈ edgesSoFar, f.node1 = ↑a ∧ f.node2 = ↑b ∨ f.node1 = ↑b ∧ f.node2 = ↑a, symm := (by simp [Symmetric]; intro a b e; grind), loopless := (by simp [irrefl_def]; intro a e _ h_eq₁ h_eq₂; have h_lt := e.nodesLt; simp [h_eq₁, h_eq₂] at h_lt) }
+        -- set H :  SimpleGraph (Fin (nodeList.max h_nonempty).id.succ) := { Adj := fun a b => (e.node1 = ↑a ∧ e.node2 = ↑b ∨ e.node1 = ↑b ∧ e.node2 = ↑a) ∨ ∃ f ∈ edgesSoFar, f.node1 = ↑a ∧ f.node2 = ↑b ∨ f.node1 = ↑b ∧ f.node2 = ↑a, symm := sorry, loopless := sorry }
+        simp at h_a_not_con
+        have h_not_reachable1 := h_invariant a ⟨e.node1, h_e1_lt_max⟩ x h_x_in h_x ⟨e.node1⟩ h_e1_in (by simp)
+        simp [ne_comm.mp h_a_not_con.left] at h_not_reachable1
+        have h_not_reachable2 := h_invariant a ⟨e.node2, h_e2_lt_max⟩ x h_x_in h_x ⟨e.node2⟩ h_e2_in (by simp)
+        simp [ne_comm.mp h_a_not_con.right] at h_not_reachable2
+        let q  := walk_of_keine_ahnung H G a b p edgesSoFar e (by simp [H]) (by simp [G]) h_not_reachable1 h_not_reachable2
+        exact ⟨q⟩
+      · intro h_cc_eq'
+        have h := (h_invariant a b x h_x_in h_x y h_y_in h_y).mpr h_cc_eq'
+        simp [SimpleGraph.Reachable]
+        by_cases h_eq : a = b
+        · simp [h_eq]
+          constructor
+          exact SimpleGraph.Walk.nil
+        · -- set G :  SimpleGraph (Fin (nodeList.max h_nonempty).id.succ) := { Adj := fun a b => ∃ f ∈ edgesSoFar, f.node1 = ↑a ∧ f.node2 = ↑b ∨ f.node1 = ↑b ∧ f.node2 = ↑a, symm := (by simp [Symmetric]; intro a b e; grind), loopless := (by simp [irrefl_def]; intro a e _ h_eq₁ h_eq₂; have h_lt := e.nodesLt; simp [h_eq₁, h_eq₂] at h_lt) }
+          -- set H :  SimpleGraph (Fin (nodeList.max h_nonempty).id.succ) := { Adj := fun a b => (e.node1 = ↑a ∧ e.node2 = ↑b ∨ e.node1 = ↑b ∧ e.node2 = ↑a) ∨ ∃ f ∈ edgesSoFar, f.node1 = ↑a ∧ f.node2 = ↑b ∨ f.node1 = ↑b ∧ f.node2 = ↑a, symm := (by simp [Symmetric]; intro a b e; grind), loopless :=  (by simp [irrefl_def]; intro a; constructor; grind; intro e _ h_eq₁ h_eq₂; have h_lt := e.nodesLt; simp [h_eq₁, h_eq₂] at h_lt) }
+          -- have h_ex_p : ∃ p, (p : G.Walk a b)
+          simp [SimpleGraph.Reachable] at h
+          cases h with
+          | intro p =>
+          let q : H.Walk a b := walk_of_subgraph G H h_subgraph a b p
+          exact ⟨q⟩
+
+theorem kruskal_helper_IsAcyclic
+  {edgeList : List edge}
+  {nodeList : List node}
+  {uF : unionFind nodeList}
+  {edgesSoFar : List edge}
+  {h_matching_edge : matching_edge edgeList nodeList}
+  {h_nodup : nodeList.Nodup}
+  (h_nonempty : nodeList ≠ [])
+  {h_symm : Symmetric fun (a b : Fin (nodeList.max h_nonempty).id.succ) => ∃ e ∈ kruskal_helper edgeList nodeList uF edgesSoFar h_matching_edge h_nodup, e.node1 = ↑a ∧ e.node2 = ↑b ∨ e.node1 = ↑b ∧ e.node2 = ↑a}
+  {h_loopless : Std.Irrefl fun (a b : Fin (nodeList.max h_nonempty).id.succ) => ∃ e ∈ kruskal_helper edgeList nodeList uF edgesSoFar h_matching_edge h_nodup, e.node1 = ↑a ∧ e.node2 = ↑b ∨ e.node1 = ↑b ∧ e.node2 = ↑a}
+  {h_symm' : Symmetric fun (a b : Fin (nodeList.max h_nonempty).id.succ) => ∃ e ∈ edgesSoFar, e.node1 = ↑a ∧ e.node2 = ↑b ∨ e.node1 = ↑b ∧ e.node2 = ↑a}
+  {h_loopless' : Std.Irrefl fun (a b : Fin (nodeList.max h_nonempty).id.succ) => ∃ e ∈ edgesSoFar, e.node1 = ↑a ∧ e.node2 = ↑b ∨ e.node1 = ↑b ∧ e.node2 = ↑a}
+  (h_matching_edge : matching_edge edgeList nodeList)
+  (h_invariant₁ : (fun (G : SimpleGraph (Fin (nodeList.max h_nonempty).id.succ)) => G.IsAcyclic) { Adj := fun a b => ∃ e ∈ edgesSoFar, e.node1 = ↑a ∧ e.node2 = ↑b ∨ e.node1 = ↑b ∧ e.node2 = ↑a, symm := h_symm', loopless := h_loopless'})
+  (h_invariant₂ : (fun (H : SimpleGraph (Fin (nodeList.max h_nonempty).id.succ)) => ∀ (a b : Fin _), (h_ex_x : ∃ x ∈ nodeList, x.id = ↑a) → (h_ex_y : ∃ x ∈ nodeList, x.id = ↑b) → H.Reachable a b ↔ connected_component_of_unionFind_of_id uF a.val h_ex_x = connected_component_of_unionFind_of_id uF b.val h_ex_y) { Adj := fun a b => ∃ e ∈ edgesSoFar, e.node1 = ↑a ∧ e.node2 = ↑b ∨ e.node1 = ↑b ∧ e.node2 = ↑a, symm := h_symm', loopless := h_loopless'})
+  : (fun (H : SimpleGraph (Fin (nodeList.max h_nonempty).id.succ)) => H.IsAcyclic) { Adj := fun a b => ∃ e ∈ kruskal_helper edgeList nodeList uF edgesSoFar h_matching_edge h_nodup, e.node1 = ↑a ∧ e.node2 = ↑b ∨ e.node1 = ↑b ∧ e.node2 = ↑a, symm := h_symm, loopless := h_loopless } := by
+  simp
+  induction
+    edgeList,
+    uF,
+    edgesSoFar,
+    h_matching_edge
+  using kruskal_helper.induct with -- generalizing h_nodeList
+  | case1 uF edgesSoFar h_matching_edge =>
+    simp [kruskal_helper]
+    exact h_invariant₁
+  | case2 uF edgesSoFar e es h_matching_edge' h_ex_1 x h_ex_2 y h_matching_edge h_uFLx =>
+    rename_i h_uFLy updated_uF updated_edgesSoFar ih
+    simp [kruskal_helper]
+    have h_x : connected_component_of_unionFind_of_id uF e.node1 (kruskal_helper._proof_1 nodeList e es h_matching_edge') = x := by
+      simp [x]
+    have h_y : connected_component_of_unionFind_of_id uF e.node2 (kruskal_helper._proof_2 nodeList e es h_matching_edge') = y := by
+      simp [y]
+    simp [h_x, h_y]
+    apply ih
+    · simp [updated_edgesSoFar, update_edgesSoFar]
+      by_cases h_eq : x = y
+      · simp [h_eq]
+        exact h_invariant₁
+      · simp [h_eq]
+        simp [matching_edge] at h_matching_edge
+        have h_match1 := h_matching_edge.left.left
+        have h_match2 := h_matching_edge.left.right
+        simp [eq_comm] at h_match1
+        simp [eq_comm] at h_match2
+        have h_e1_lt : e.node1 < (nodeList.max h_nonempty).id.succ := by
+          rcases h_match1 with ⟨z, h_z⟩
+          simp [← h_z.right]
+          have h_goal : z ≤ nodeList.max h_nonempty := by
+            grind
+          exact h_goal
+        have h_e2_lt : e.node2 < (nodeList.max h_nonempty).id.succ := by
+          rcases h_match2 with ⟨z, h_z⟩
+          simp [← h_z.right]
+          have h_goal : z ≤ nodeList.max h_nonempty := by
+            grind
+          exact h_goal
+        set G : SimpleGraph (Fin (nodeList.max h_nonempty).id.succ) := { Adj := fun a b => ∃ e ∈ edgesSoFar, e.node1 = ↑a ∧ e.node2 = ↑b ∨ e.node1 = ↑b ∧ e.node2 = ↑a, symm := h_symm', loopless := h_loopless' } with ← h_G
+        have h_not_reachable : ¬G.Reachable ⟨e.node1, h_e1_lt⟩ ⟨e.node2, h_e2_lt⟩ := by
+          intro h
+          have h' := (h_invariant₂ ⟨e.node1, h_e1_lt⟩ ⟨e.node2, h_e2_lt⟩ h_match1 h_match2).mp h
+          simp [h_x, h_y, h_eq] at h'
+        have h := (SimpleGraph.isAcyclic_add_edge_iff_of_not_reachable _ _ h_not_reachable).mpr h_invariant₁
+        have h_symm'' : Symmetric fun (a b : Fin (nodeList.max h_nonempty).id.succ) => (e.node1 = ↑a ∧ e.node2 = ↑b ∨ e.node1 = ↑b ∧ e.node2 = ↑a) ∨ ∃ a_1 ∈ edgesSoFar, a_1.node1 = ↑a ∧ a_1.node2 = ↑b ∨ a_1.node1 = ↑b ∧ a_1.node2 = ↑a := by
+          simp [Symmetric]
+          intro a b e
+          grind
+        have h_loopless'' : Std.Irrefl fun (a b : Fin (nodeList.max h_nonempty).id.succ) => (e.node1 = ↑a ∧ e.node2 = ↑b ∨ e.node1 = ↑b ∧ e.node2 = ↑a) ∨ ∃ a_1 ∈ edgesSoFar, a_1.node1 = ↑a ∧ a_1.node2 = ↑b ∨ a_1.node1 = ↑b ∧ a_1.node2 = ↑a := by
+          simp [irrefl_def]
+          intro a
+          constructor
+          · grind
+          · intro e _ h_eq₁ h_eq₂
+            have h_lt := e.nodesLt
+            simp [h_eq₁, h_eq₂] at h_lt
+        have h_add_edge_eq : G ⊔ SimpleGraph.edge ⟨e.node1, h_e1_lt⟩ ⟨e.node2, h_e2_lt⟩ = { Adj := fun a b => (e.node1 = ↑a ∧ e.node2 = ↑b ∨ e.node1 = ↑b ∧ e.node2 = ↑a) ∨ ∃ a_1 ∈ edgesSoFar, a_1.node1 = ↑a ∧ a_1.node2 = ↑b ∨ a_1.node1 = ↑b ∧ a_1.node2 = ↑a, symm := h_symm'', loopless := h_loopless'' } := by
+          simp [G]
+          ext a b
+          simp [SimpleGraph.edge]
+          grind
+        simp [h_add_edge_eq] at h
+        exact h
+    · simp [updated_edgesSoFar, update_edgesSoFar, updated_uF]
+      by_cases h_eq : x = y
+      · simp [h_eq, update_unionFind]
+        simp at h_invariant₂
+        exact h_invariant₂
+      · intro a b xa h_xa_in h_xa xb h_xb_in h_xb
+        simp [h_eq]
+        simp at h_invariant₂
+        have h := kruskal_helper_Reachable_iff_con h_nonempty h_ex_1 h_ex_2 h_uFLx h_uFLy (by simp; exact h_invariant₂) a b ⟨xa, h_xa_in, h_xa⟩ ⟨xb, h_xb_in, h_xb⟩ (h_nodup := h_nodup) (h_matching_edge := h_matching_edge) (edgesSoFar := edgesSoFar) (uF := uF) (e := e)
+        simp [update_edgesSoFar, h_x, h_y, h_eq] at h
+        exact h
+    · simp [Symmetric]
+      intro a b e
+      grind
+    · simp [irrefl_def]
+      intro a e _ h_eq₁ h_eq₂
+      have h_lt := e.nodesLt
+      simp [h_eq₁, h_eq₂] at h_lt
+
+-- nicht von mir gelöst sondern von Zulip-Nutzer Aaron Liu https://leanprover.zulipchat.com/#user/816344
+theorem cast_Fin_fun {n m : Nat} {a b : Fin m} (f : (Fin n) → (Fin n) → Prop) (h : Fin n = Fin m) : (h ▸ f) a b = f (h ▸ a) (h ▸ b) := by
+  cases fin_injective h
+  rfl
+
+theorem SimpleGraph_of_kruskal.IsAcyclic (edgeList : List edge) (h : edgeList ≠ []) : (SimpleGraph_of_kruskal edgeList h).IsAcyclic := by
+  set G := SimpleGraph_of_kruskal edgeList h with h_G
+  simp [SimpleGraph_of_kruskal, SimpleGraph_of_n_of_edgeList, SimpleGraph_of_edgeList, kruskal_of_edgeList, kruskal] at h_G --, SimpleGraph.Walk.isCycle_iff_isPath_tail_and_le_length]
+  set edgeListSorted := edgeList.mergeSort fun a b => decide (a ≤ b) with h_edgeListSorted
+  set nodeList := nodeList_of_edgeList edgeList with h_nodeList
+  set uF := init_unionFind (nodeList_of_edgeList edgeList) (nodeList_of_edgeList_nodup edgeList) with h_uF
+  set edgesSoFar : List edge := [] with h_edgesSoFar
+  simp [h_edgesSoFar] at h
+  have h_matching_edge : matching_edge _ _ := kruskal._proof_1 edgeList (nodeList_of_edgeList edgeList) (matching_edge_for_nodeList_of_edgeList edgeList)
+  have h_nodup := nodeList_of_edgeList_nodup edgeList
+  simp [← h_edgeListSorted, ← h_uF, ← h_edgesSoFar] at h_G
+  have h_eq := nodeList_of_edgeList_max_eq edgeList h
+  simp only [kruskal_of_edgeList, kruskal, Nat.succ_eq_add_one] at h_eq
+  nth_rewrite 2 [nodeList_of_edgeList_max] at h_eq
+  -- rw [h_eq]
+  have h_nonempty : nodeList ≠ [] := by
+    exact nodeList_of_edgeList_nonempty edgeList h
+  have h_symm : Symmetric fun (a b : Fin (nodeList.max h_nonempty).id.succ) => ∃ e ∈ kruskal_helper edgeListSorted nodeList uF edgesSoFar h_matching_edge h_nodup, e.node1 = ↑a ∧ e.node2 = ↑b ∨ e.node1 = ↑b ∧ e.node2 = ↑a := by
+    simp [Symmetric]
+    intro a b e
+    grind
+  have h_loopless : Std.Irrefl fun (a b : Fin (nodeList.max h_nonempty).id.succ) => ∃ e ∈ kruskal_helper edgeListSorted nodeList uF edgesSoFar h_matching_edge h_nodup, e.node1 = ↑a ∧ e.node2 = ↑b ∨ e.node1 = ↑b ∧ e.node2 = ↑a := by
+    simp [irrefl_def]
+    intro a e _ h_eq₁ h_eq₂
+    have h_lt := e.nodesLt
+    simp [h_eq₁, h_eq₂] at h_lt
+  have h_symm' : Symmetric fun (a b : Fin (nodeList.max h_nonempty).id.succ) => ∃ e ∈ edgesSoFar, e.node1 = ↑a ∧ e.node2 = ↑b ∨ e.node1 = ↑b ∧ e.node2 = ↑a := by
+    simp [Symmetric]
+    intro a b e
+    grind
+  have h_loopless' : Std.Irrefl fun (a b : Fin (nodeList.max h_nonempty).id.succ) => ∃ e ∈ edgesSoFar, e.node1 = ↑a ∧ e.node2 = ↑b ∨ e.node1 = ↑b ∧ e.node2 = ↑a := by
+    simp [irrefl_def]
+    intro a e _ h_eq₁ h_eq₂
+    have h_lt := e.nodesLt
+    simp [h_eq₁, h_eq₂] at h_lt
+  have h_acyclic_of_invariants := kruskal_helper_IsAcyclic h_nonempty h_matching_edge (edgeList := edgeListSorted) (nodeList := nodeList_of_edgeList edgeList) (uF := uF) (edgesSoFar := edgesSoFar) (h_nodup := h_nodup) (h_matching_edge := h_matching_edge) (h_loopless := h_loopless) (h_loopless' := h_loopless') (h_symm := h_symm) (h_symm' := h_symm')
+  simp at h_acyclic_of_invariants
+  have h_acyclic := h_acyclic_of_invariants ?_ ?_
+  · have h_SimpleGraph_eq : SimpleGraph (Fin ((nodeList_of_edgeList edgeList).max (nodeList_of_edgeList_nonempty edgeList h)).id.succ) = SimpleGraph (Fin (nodeList_of_edgeList_max (kruskal_of_edgeList edgeList) (kruskal_nonempty _ h)).id.succ) := by
+      simp [← h_eq, nodeList_of_edgeList_max, kruskal_of_edgeList, kruskal]
+    have h_Fin_eq : Fin ((nodeList_of_edgeList edgeList).max (nodeList_of_edgeList_nonempty edgeList h)).id.succ = Fin (nodeList_of_edgeList_max (kruskal_of_edgeList edgeList) (kruskal_nonempty _ h)).id.succ := by
+      simp [← h_eq, nodeList_of_edgeList_max, kruskal_of_edgeList, kruskal]
+    set H : SimpleGraph (Fin (((nodeList_of_edgeList edgeList).max (nodeList_of_edgeList_nonempty edgeList h)).id + 1)) := { Adj := fun a b => ∃ e ∈ kruskal_helper edgeListSorted (nodeList_of_edgeList edgeList) uF edgesSoFar h_matching_edge h_nodup, e.node1 = ↑a ∧ e.node2 = ↑b ∨ e.node1 = ↑b ∧ e.node2 = ↑a, symm := h_symm, loopless := h_loopless } with h_H
+    set G' := h_Fin_eq ▸ H with ← h_G'
+    have : G'.IsAcyclic := by
+      grind
+    have : G = G' := by
+      simp [h_G, G']
+      ext a b
+      have h_cast_1 : (h_Fin_eq ▸ H).Adj = h_Fin_eq ▸ H.Adj := by
+        grind
+      have h_cast_2 : (h_Fin_eq ▸ H.Adj) a b = H.Adj (h_Fin_eq ▸ a) (h_Fin_eq ▸ b) := by
+        apply cast_Fin_fun
+      simp [h_cast_1, h_cast_2]
+      simp [H]
+      have h_cast_3 : (h_Fin_eq ▸ a).val = a.val := by
+        grind
+      have h_cast_4 : (h_Fin_eq ▸ b).val = b.val := by
+        grind
+      simp [h_cast_3, h_cast_4]
+    grind
+  · simp [edgesSoFar, SimpleGraph.isAcyclic_iff_forall_adj_isBridge]
+  · simp [edgesSoFar]
+    intro a b x h_x_in h_x y h_y_in h_y
+    constructor
+    · simp [SimpleGraph.Reachable]
+      intro p
+      cases p with
+      | nil =>
+        simp
+      | cons h_adj p' =>
+        simp at h_adj
+    · simp [nodeList] at h_nonempty
+      simp [connected_component_of_unionFind_of_id]
+      set uFLa := List.choose (fun x => x.nodeId = ↑a) uF.linkList (connected_component_of_unionFind_of_id._proof_1 uF (↑a) (Exists.intro x ⟨h_x_in, h_x⟩)) with ← h_uFLa
+      set uFLb := List.choose (fun x => x.nodeId = ↑b) uF.linkList (connected_component_of_unionFind_of_id._proof_1 uF (↑b) (Exists.intro y ⟨h_y_in, h_y⟩)) with ← h_uFLb
+      simp [h_uFLa, h_uFLb]
+      have h_uFLa_mem := List.choose_mem (fun x => x.nodeId = ↑a) uF.linkList (connected_component_of_unionFind_of_id._proof_1 uF (↑a) (Exists.intro x ⟨h_x_in, h_x⟩))
+      have h_uFLb_mem := List.choose_mem (fun x => x.nodeId = ↑b) uF.linkList (connected_component_of_unionFind_of_id._proof_1 uF (↑b) (Exists.intro y ⟨h_y_in, h_y⟩))
+      have h_uFLa_prop := List.choose_property (fun x => x.nodeId = ↑a) uF.linkList (connected_component_of_unionFind_of_id._proof_1 uF (↑a) (Exists.intro x ⟨h_x_in, h_x⟩))
+      have h_uFLb_prop := List.choose_property (fun x => x.nodeId = ↑b) uF.linkList (connected_component_of_unionFind_of_id._proof_1 uF (↑b) (Exists.intro y ⟨h_y_in, h_y⟩))
+      simp [h_uFLa, h_uFLb] at h_uFLa_mem h_uFLb_mem h_uFLa_prop h_uFLb_prop
+      simp [uF, init_unionFind, h_nonempty, init_unionFind.linkList] at h_uFLa_mem h_uFLb_mem
+      have h_all_self_con := init_unionFind.linkList.helper_all_self_connected (nodeList_of_edgeList edgeList) (nodeList_of_edgeList edgeList) (by simp [h_nonempty])
+      rw [connected_component_of_unionFind_of_unionFindLink]
+      rw [connected_component_of_unionFind_of_unionFindLink]
+      simp [← h_all_self_con uFLa h_uFLa_mem, ← h_all_self_con uFLb h_uFLb_mem, h_uFLa_prop, h_uFLb_prop]
+      intro h_a_eq_b
+      have h_a_eq_b : a = b := by
+        cases a
+        cases b
+        simp at h_a_eq_b
+        simp [h_a_eq_b]
+      simp [h_a_eq_b]
+
+instance fin_of_edgeList_Finite {edgeList : List edge} {h : edgeList ≠ []} : Finite (fin_of_edgeList edgeList h) := by
+  simp [fin_of_edgeList]
+  exact Finite.of_fintype (Fin ((nodeList_of_edgeList_max edgeList h).id + 1))
+
+noncomputable instance SimpleGraph_of_edgeList.edgeSet_Fintype {edgeList : List edge} {h : edgeList ≠ []} : Fintype ↑(SimpleGraph_of_edgeList edgeList h).edgeSet :=
+  Fintype.ofFinite ↑(SimpleGraph_of_edgeList edgeList h).edgeSet
+
+theorem SimpleGraph_of_edgeList.ex_edge_of_edge (edgeList : List edge) (h : edgeList ≠ []) : ∀ (a b : fin_of_edgeList edgeList h), s(a, b) ∈ (SimpleGraph_of_edgeList edgeList h).edgeFinset → ∃ e ∈ edgeList, e.node1 = a.val ∧ e.node2 = b.val ∨ e.node1 = b.val ∧ e.node2 = a.val := by
+  intro a b h_s_in
+  simp [SimpleGraph_of_edgeList] at h_s_in
+  exact h_s_in
+
+noncomputable def SimpleGraph_of_edgeList.edge_of_edge (edgeList : List edge) (h : edgeList ≠ []) : (SimpleGraph_of_edgeList edgeList h).edgeFinset → edgeList.toFinset := by
+  intro s -- a b h_s_in
+  rcases s with ⟨s, h_s_in⟩
+  simp [Sym2] at s
+  -- have h_ex_s' := s.exists_rep
+  have h_ex_a_b: ∃ a b, s = s(a, b) := by
+    rcases s with ⟨a, b⟩
+    refine ⟨a, b, rfl⟩
+    -- rcases h_ex_s' with ⟨s', h⟩
+    -- simp at h_s_in
+  set a := Classical.choose h_ex_a_b with ← h_a
+  have h_a_spec := Classical.choose_spec h_ex_a_b
+  set b := Classical.choose h_a_spec with ← h_b
+  have h_b_spec := Classical.choose_spec h_a_spec
+  simp [h_a, h_b] at h_b_spec
+  simp only [h_b_spec] at h_s_in
+  have h_ex_edge_of_edge := SimpleGraph_of_edgeList.ex_edge_of_edge edgeList h a b h_s_in
+  let e := List.choose (fun (e : edge) => e.node1 = a.val ∧ e.node2 = b.val ∨ e.node1 = b.val ∧ e.node2 = a.val) edgeList h_ex_edge_of_edge
+  have h_e_in := List.choose_mem (fun (e : edge) => e.node1 = a.val ∧ e.node2 = b.val ∨ e.node1 = b.val ∧ e.node2 = a.val) edgeList h_ex_edge_of_edge
+  have h_e_in' : e ∈ edgeList.toFinset := by
+    exact List.mem_toFinset.mpr h_e_in
+  exact ⟨e, h_e_in'⟩
+
+theorem SimpleGraph_of_edgeList.edge_of_edge_injective (edgeList : List edge) (h : edgeList ≠ []) : Function.Injective (SimpleGraph_of_edgeList.edge_of_edge edgeList h) := by
+  intro s1 s2 h_eq
+  simp [SimpleGraph_of_edgeList.edge_of_edge] at h_eq
+  set a := Classical.choose (SimpleGraph_of_edgeList.edge_of_edge._proof_1 edgeList h (↑s1) s1.property) with ← h_a
+  set b := Classical.choose (SimpleGraph_of_edgeList.edge_of_edge._proof_3 edgeList h (↑s1) (edge_of_edge._proof_1 edgeList h (↑s1) s1.property)) with ← h_b
+  set c := Classical.choose (SimpleGraph_of_edgeList.edge_of_edge._proof_1 edgeList h (↑s2) s2.property) with ← h_c
+  set d := Classical.choose (SimpleGraph_of_edgeList.edge_of_edge._proof_3 edgeList h (↑s2) (edge_of_edge._proof_1 edgeList h (↑s2) s2.property)) with ← h_d
+  have h_a_prop := Classical.choose_spec (SimpleGraph_of_edgeList.edge_of_edge._proof_1 edgeList h (↑s1) s1.property)
+  have h_b_prop := Classical.choose_spec (SimpleGraph_of_edgeList.edge_of_edge._proof_3 edgeList h (↑s1) (edge_of_edge._proof_1 edgeList h (↑s1) s1.property))
+  have h_c_prop := Classical.choose_spec (SimpleGraph_of_edgeList.edge_of_edge._proof_1 edgeList h (↑s2) s2.property)
+  have h_d_prop := Classical.choose_spec (SimpleGraph_of_edgeList.edge_of_edge._proof_3 edgeList h (↑s2) (edge_of_edge._proof_1 edgeList h (↑s2) s2.property))
+  simp [h_a, h_b, h_c, h_d] at h_eq h_a_prop h_b_prop h_c_prop h_d_prop
+  have h_ex_e1 : ∃ e ∈ edgeList, e.node1 = a.val ∧ e.node2 = b.val ∨ e.node1 = b.val ∧ e.node2 = a.val := by
+    have h_ex_a_b : ∃ (a b : fin_of_edgeList edgeList h), s1 = s(a, b) := by refine ⟨a, b, h_b_prop⟩
+    have h := (SimpleGraph_of_edgeList.edge_of_edge._proof_6 edgeList h (↑s1) s1.property) h_ex_a_b rfl h_a_prop rfl h_b_prop
+    exact h
+  have h_ex_e2 : ∃ e ∈ edgeList, e.node1 = c.val ∧ e.node2 = d.val ∨ e.node1 = d.val ∧ e.node2 = c.val := by
+    have h_ex_a_b : ∃ (c d : fin_of_edgeList edgeList h), s2 = s(c, d) := by refine ⟨c, d, h_d_prop⟩
+    have h := (SimpleGraph_of_edgeList.edge_of_edge._proof_6 edgeList h (↑s2) s2.property) h_ex_a_b rfl h_c_prop rfl h_d_prop
+    exact h
+  set e1 := List.choose (fun e => e.node1 = a.val ∧ e.node2 = b.val ∨ e.node1 = b.val ∧ e.node2 = a.val) edgeList h_ex_e1 with ← h_e1
+  set e2 := List.choose (fun e => e.node1 = c.val ∧ e.node2 = d.val ∨ e.node1 = d.val ∧ e.node2 = c.val) edgeList h_ex_e2 with ← h_e2
+  have h_e1_prop := List.choose_property (fun e => e.node1 = a.val ∧ e.node2 = b.val ∨ e.node1 = b.val ∧ e.node2 = a.val) edgeList h_ex_e1
+  have h_e2_prop := List.choose_property (fun e => e.node1 = c.val ∧ e.node2 = d.val ∨ e.node1 = d.val ∧ e.node2 = c.val) edgeList h_ex_e2
+  simp [h_e1, h_e2, h_eq] at h_e1_prop h_e2_prop
+  have h_goal : s(a, b) = s(c, d) := by
+    rcases h_e1_prop with h_e1_prop | h_e1_prop
+    · rcases h_e2_prop with h_e2_prop | h_e2_prop
+      · simp [h_e1_prop] at h_e2_prop
+        simp
+        grind
+      · simp [h_e1_prop] at h_e2_prop
+        simp
+        grind
+    · rcases h_e2_prop with h_e2_prop | h_e2_prop
+      · simp [h_e1_prop] at h_e2_prop
+        simp
+        grind
+      · simp [h_e1_prop] at h_e2_prop
+        simp
+        grind
+  simp [h_goal, ← h_d_prop] at h_b_prop
+  exact h_b_prop
+
+def SimpleGraph_of_edgeList.edge_of_edge_reverse (edgeList : List edge) (h : edgeList ≠ []) : edgeList.toFinset → (SimpleGraph_of_edgeList edgeList h).edgeFinset := by
+  intro e -- h_e_in
+  rcases e with ⟨e, h_e_in⟩
+  have h_e_in : e ∈ edgeList := List.mem_dedup.mp h_e_in
+  have h_lt1 : e.node1 < (nodeList_of_edgeList_max edgeList h).id.succ := by
+    have h_goal : ⟨e.node1⟩ ≤ nodeList_of_edgeList_max edgeList h := by
+      simp [nodeList_of_edgeList_max]
+      have h_matching_edge := matching_edge_for_nodeList_of_edgeList edgeList
+      simp [matching_edge] at h_matching_edge
+      have h_matching_edge := (h_matching_edge e h_e_in).left
+      rcases h_matching_edge with ⟨x, h_x_in, h_x⟩
+      cases x
+      simp at h_x
+      simp [← h_x] at h_x_in
+      simp [List.le_max_of_mem h_x_in]
+    simp
+    exact h_goal
+  have h_lt2 : e.node2 < (nodeList_of_edgeList_max edgeList h).id.succ := by
+    have h_goal : ⟨e.node2⟩ ≤ nodeList_of_edgeList_max edgeList h := by
+      simp [nodeList_of_edgeList_max]
+      have h_matching_edge := matching_edge_for_nodeList_of_edgeList edgeList
+      simp [matching_edge] at h_matching_edge
+      have h_matching_edge := (h_matching_edge e h_e_in).right
+      rcases h_matching_edge with ⟨x, h_x_in, h_x⟩
+      cases x
+      simp at h_x
+      simp [← h_x] at h_x_in
+      simp [List.le_max_of_mem h_x_in]
+    simp
+    exact h_goal
+  let a : fin_of_edgeList edgeList h := ⟨e.node1, h_lt1⟩
+  let b : fin_of_edgeList edgeList h := ⟨e.node2, h_lt2⟩
+  have h_edge : s(a, b) ∈ (SimpleGraph_of_edgeList edgeList h).edgeFinset := by
+    simp [SimpleGraph_of_edgeList]
+    simp [a, b]
+    refine ⟨e, h_e_in, by simp⟩
+  set s := s(a, b)
+  exact ⟨s, h_edge⟩
+
+theorem SimpleGraph_of_edgeList.edge_of_edge_reverse_injective
+  (edgeList : List edge) (h : edgeList ≠ []) (h_nodup_con : ∀ e1 ∈ edgeList, ∀ e2 ∈ edgeList, e1.node1 = e2.node1 ∧ e1.node2 = e2.node2 ∨ e1.node1 = e2.node2 ∧ e1.node2 = e2.node1 → e1 = e2)
+  : Function.Injective (SimpleGraph_of_edgeList.edge_of_edge_reverse edgeList h) := by
+  intro e₁ e₂ h_eq
+  rcases e₁ with ⟨e₁, h_e₁_in⟩
+  rcases e₂ with ⟨e₂, h_e₂_in⟩
+  have h_e₁_in : e₁ ∈ edgeList := List.mem_dedup.mp h_e₁_in
+  have h_e₂_in : e₂ ∈ edgeList := List.mem_dedup.mp h_e₂_in
+  simp [SimpleGraph_of_edgeList.edge_of_edge_reverse] at h_eq
+  have h_eq : e₁.node1 = e₂.node1 ∧ e₁.node2 = e₂.node2 ∨ e₁.node1 = e₂.node2 ∧ e₁.node2 = e₂.node1 := by
+    grind
+  exact Subtype.ext <| h_nodup_con e₁ h_e₁_in e₂ h_e₂_in h_eq
+
+theorem SimpleGraph_of_edgeList.card_edgeSet_eq_edgeList_length (edgeList : List edge) (h : edgeList ≠ []) (h_nodup_con : ∀ e1 ∈ edgeList, ∀ e2 ∈ edgeList, e1.node1 = e2.node1 ∧ e1.node2 = e2.node2 ∨ e1.node1 = e2.node2 ∧ e1.node2 = e2.node1 → e1 = e2) (h_nodup : edgeList.Nodup) : (SimpleGraph_of_edgeList edgeList h).edgeFinset.card = edgeList.length := by
+  have h_card_sub : edgeList.toFinset.card = edgeList.length := by
+    exact List.toFinset_card_of_nodup h_nodup
+  have h_le : (SimpleGraph_of_edgeList edgeList h).edgeFinset.card ≤ edgeList.length := by
+    have h' := Fintype.card_le_of_injective (SimpleGraph_of_edgeList.edge_of_edge edgeList h) (SimpleGraph_of_edgeList.edge_of_edge_injective edgeList h)
+    simp only [Fintype.card_coe, h_card_sub] at h'
+    exact h'
+  have h_ge : (SimpleGraph_of_edgeList edgeList h).edgeFinset.card ≥ edgeList.length := by
+    have h' := Fintype.card_le_of_injective (SimpleGraph_of_edgeList.edge_of_edge_reverse edgeList h) (SimpleGraph_of_edgeList.edge_of_edge_reverse_injective edgeList h h_nodup_con)
+    simp only [Fintype.card_coe, h_card_sub] at h'
+    exact h'
+  exact eq_of_le_of_ge h_le h_ge
+
+instance (edgeList : List edge) (h : edgeList ≠ []) : Fintype (fin_of_edgeList edgeList h) := by
+  simp [fin_of_edgeList]
+  exact Fin.fintype ((nodeList_of_edgeList_max edgeList h).id + 1)
+
+instance (edgeList : List edge) (h : edgeList ≠ []) : Nonempty (fin_of_edgeList edgeList h) := by
+  simp [fin_of_edgeList]
+  exact instNonemptyOfInhabited
+
+theorem SimpleGraph_of_edgeList.card_edgeSet (edgeList : List edge) (h : edgeList ≠ []) (h_nodup_con : ∀ e1 ∈ edgeList, ∀ e2 ∈ edgeList, e1.node1 = e2.node1 ∧ e1.node2 = e2.node2 ∨ e1.node1 = e2.node2 ∧ e1.node2 = e2.node1 → e1 = e2) (h_nodup : edgeList.Nodup) (h_acyclic : (SimpleGraph_of_edgeList edgeList h).IsAcyclic) : edgeList.length < (nodeList_of_edgeList_max edgeList h).id.succ := by
+  have h_eq : (nodeList_of_edgeList_max edgeList h).id.succ = Fintype.card (fin_of_edgeList edgeList h) := by
+    simp [fin_of_edgeList]
+    exact Eq.symm (Fintype.card_fin ((nodeList_of_edgeList_max edgeList h).id + 1))
+  simp only [h_eq]
+  have h_tantow := h_acyclic.card_edgeFinset_le
+  simp at h_tantow
+  apply lt_of_eq_of_lt ?_ h_tantow
+  exact (SimpleGraph_of_edgeList.card_edgeSet_eq_edgeList_length edgeList h h_nodup_con h_nodup).symm
+
+-- geht auch ohne edgeList.Nodup, ist aber aufwändiger
+theorem kruskal_helper.Nodup (edgeList : List edge) (nodeList : List node) (uF : unionFind nodeList) (edgesSoFar : List edge) (h_matching_edge : matching_edge edgeList nodeList) (h_nodup : nodeList.Nodup) (h_invariant : (edgeList ++ edgesSoFar).Nodup) : (kruskal_helper edgeList nodeList uF edgesSoFar h_matching_edge h_nodup).Nodup := by
+  fun_induction kruskal_helper with
+  | case1 uF edgesSoFar h_matching_edge =>
+    exact h_invariant
+  | case2 uF edgesSoFar e es h_matching_edge h x h' y h_matching_edge' h_x h_y updated_uF updated_edgesSoFar ih =>
+    apply ih
+    simp [updated_edgesSoFar, update_edgesSoFar]
+    split_ifs
+    · grind
+    · grind
+
+-- geht auch ohne edgeList.Nodup, abhängig von kruskal_helper.Nodup
+theorem kruskal_of_edgeList.Nodup (edgeList : List edge) (h_nodup : edgeList.Nodup) : (kruskal_of_edgeList edgeList).Nodup := by
+  simp [kruskal_of_edgeList, kruskal]
+  apply kruskal_helper.Nodup
+  simp [h_nodup]
+
+-- geht auch ohne edgeList.nodup_con, ist aber aufwändiger
+theorem kruskal_helper.nodup_con (edgeList : List edge) (nodeList : List node) (uF : unionFind nodeList) (edgesSoFar : List edge) (h_matching_edge : matching_edge edgeList nodeList) (h_nodup : nodeList.Nodup) (h_invariant : ∀ e1 ∈ edgeList ++ edgesSoFar, ∀ e2 ∈ edgeList ++ edgesSoFar, e1.node1 = e2.node1 ∧ e1.node2 = e2.node2 ∨ e1.node1 = e2.node2 ∧ e1.node2 = e2.node1 → e1 = e2) : ∀ e1 ∈ (kruskal_helper edgeList nodeList uF edgesSoFar h_matching_edge h_nodup), ∀ e2 ∈ (kruskal_helper edgeList nodeList uF edgesSoFar h_matching_edge h_nodup), e1.node1 = e2.node1 ∧ e1.node2 = e2.node2 ∨ e1.node1 = e2.node2 ∧ e1.node2 = e2.node1 → e1 = e2 := by
+  fun_induction kruskal_helper with
+  | case1 uF edgesSoFar h_matching_edge =>
+    exact h_invariant
+  | case2 uF edgesSoFar e es h_matching_edge h x h' y h_matching_edge' h_x h_y updated_uF updated_edgesSoFar ih =>
+    apply ih
+    simp [updated_edgesSoFar, update_edgesSoFar]
+    split_ifs
+    · grind
+    · grind
+
+-- geht auch ohne edgeList.nodup_con, abhängig von kruskal_helper.nodup_con
+theorem kruskal_of_edgeList.nodup_con (edgeList : List edge) (h_nodup_con : ∀ e1 ∈ edgeList, ∀ e2 ∈ edgeList, e1.node1 = e2.node1 ∧ e1.node2 = e2.node2 ∨ e1.node1 = e2.node2 ∧ e1.node2 = e2.node1 → e1 = e2) : ∀ e1 ∈ kruskal_of_edgeList edgeList, ∀ e2 ∈ kruskal_of_edgeList edgeList, e1.node1 = e2.node1 ∧ e1.node2 = e2.node2 ∨ e1.node1 = e2.node2 ∧ e1.node2 = e2.node1 → e1 = e2 := by
+  simp [kruskal_of_edgeList, kruskal]
+  apply kruskal_helper.nodup_con
+  simp
+  exact h_nodup_con
+
+-- geht auch ohne edgeList.Nodup, abhängig von kruskal_helper.Nodup
+-- geht auch ohne edgeList.nodup_con, abhängig von kruskal_helper.nodup_con
+theorem kruskal_of_edgeList.card_edgeSet (edgeList : List edge) (h : edgeList ≠ []) (h_nodup : edgeList.Nodup) (h_nodup_con : ∀ e1 ∈ edgeList, ∀ e2 ∈ edgeList, e1.node1 = e2.node1 ∧ e1.node2 = e2.node2 ∨ e1.node1 = e2.node2 ∧ e1.node2 = e2.node1 → e1 = e2) : (kruskal_of_edgeList edgeList).length < (nodeList_of_edgeList_max (kruskal_of_edgeList edgeList) (kruskal_nonempty edgeList h)).id.succ := SimpleGraph_of_edgeList.card_edgeSet (kruskal_of_edgeList edgeList) (kruskal_nonempty edgeList h) (kruskal_of_edgeList.nodup_con edgeList h_nodup_con) (kruskal_of_edgeList.Nodup edgeList h_nodup) (by exact SimpleGraph_of_kruskal.IsAcyclic edgeList h)
+
+theorem rank_le_rank_of_mem_get_parent_path
+  {nodeList : List node}
+  {uF : unionFind nodeList}
+  {uFL uFL' : unionFindLink nodeList}
+  (h_in : uFL ∈ uF.linkList)
+  (h_in' : uFL' ∈ get_parent_path h_in)
+  (h_ne : uFL ≠ uFL')
+  : uFL.rank < uFL'.rank := by
+  fun_induction get_parent_path with
+  | case1 uFL h_in h_self_con =>
+    simp at h_in'
+    simp [h_in'] at h_ne
+  | case2 uFL h_in h_self_con ih =>
+    rw [get_parent_path] at h_in'
+    set p := parent uFL h_in with ← h_p
+    simp [h_p, ne_comm.mp h_ne] at h_in'
+    revert h_in'
+    split_ifs with h_p_self_con
+    · simp
+      intro h_in'
+      simp [h_in', p, parent]
+      have h := uF.matching_rank uFL h_in
+      simp [h_self_con] at h
+      exact h
+    · simp
+      intro h_in'
+      have h_lt_parent : uFL.rank < p.rank := by
+        simp [p, parent]
+        have h := uF.matching_rank uFL h_in
+        simp [h_self_con] at h
+        exact h
+      by_cases h_eq : uFL' = p
+      · simp [h_eq]
+        exact h_lt_parent
+      · simp [h_p] at ih
+        simp [h_eq] at h_in'
+        -- have ih := ih h_in'
+        apply lt_trans h_lt_parent
+        apply ih
+        · rw [get_parent_path]
+          simp [h_p_self_con, h_eq, h_in']
+        · exact ne_comm.mp h_eq
+
+theorem not_self_con_of_mem_get_parent_path
+  {nodeList : List node}
+  {uF : unionFind nodeList}
+  {uFL uFL' : unionFindLink nodeList}
+  (h_in : uFL ∈ uF.linkList)
+  (h_in' : uFL' ∈ get_parent_path h_in)
+  (h_ne : uFL ≠ uFL')
+  : uFL.nodeId ≠ uFL.ccId := by
+  intro h_self_con
+  rw [get_parent_path] at h_in'
+  simp [h_self_con, ne_comm.mp h_ne] at h_in'
+
+theorem le_two_pow_minus_one (n : Nat) : n ≤ 2^n-1 := by
+  induction n with
+  | zero =>
+    simp
+  | succ n ih =>
+    simp
+    apply Nat.lt_of_succ_le
+    apply Nat.le_of_lt_succ
+    have h : (2 ^ (n + 1) - 1).succ = 2 ^ (n + 1) := by
+      grind
+    rw [h]
+    exact Nat.lt_two_pow_self
+
+def unionFind.rankInvariant_strict {nodeList : List node} (uF : unionFind nodeList) := ∀ uFL ∈ uF.linkList, (uF.linkList.filter (fun x => if h_x_in : x ∈ uF.linkList then uFL ∈ get_parent_path (uFL := x) (uF := uF) h_x_in else False)).length ≥ 2^(uFL.rank.val)
+
+theorem unionFind.rankInvariant_of_rankInvariant_strict {nodeList : List node} {uF : unionFind nodeList} (h_rankInvariant : uF.rankInvariant_strict) : ∀ uFL ∈ uF.linkList, (uF.linkList.filter (fun x => x.rank < uFL.rank ∧ ¬x.nodeId = x.ccId)).length ≥ uFL.rank := by
+  intro uFL h_in
+  -- rcases uFL with ⟨nodeId, ccId, rank⟩
+  -- rcases rank with ⟨rank, h_lt⟩
+  set rank := uFL.rank.val with ← h_rank
+  revert h_rank
+  induction rank generalizing uFL with
+  | zero =>
+    simp
+  | succ rank' ih =>
+    intro h_rank'
+    have h : rank' + 1 ≤ 2^rank'-1+1 := by
+      simp [le_two_pow_minus_one rank']
+    apply le_trans h
+    have h_length_lt : (List.filter (fun x => if h_x_in : x ∈ uF.linkList then decide (uFL ∈ get_parent_path h_x_in) else decide False) uF.linkList).length ≤ (uFL :: List.filter (fun x => decide (x.rank < uFL.rank) && !decide (x.nodeId = x.ccId)) uF.linkList).length := by
+      apply nodup_length_le_length_all_mem (by simp [List.Nodup.filter, uF.nodup])
+      intro x h_x_in_filter
+      by_cases h_eq : x = uFL
+      · simp [h_eq]
+      · have h_x_in := List.mem_of_mem_filter h_x_in_filter
+        have h_x_prop := (List.mem_filter.mp h_x_in_filter).right
+        simp at h_x_prop
+        rcases h_x_prop with ⟨_, h_x_prop⟩
+        simp [h_eq, h_x_in]
+        constructor
+        · exact rank_le_rank_of_mem_get_parent_path h_x_in h_x_prop h_eq
+        · exact not_self_con_of_mem_get_parent_path h_x_in h_x_prop h_eq
+    simp at h_length_lt
+    apply Nat.le_of_lt_succ
+    apply Nat.lt_of_succ_le
+    simp only [Nat.succ_eq_add_one, Bool.decide_and, decide_not]
+    apply le_trans ?_ h_length_lt
+    apply le_trans ?_ (h_rankInvariant uFL h_in)
+    simp [h_rank']
+    have h : (2 ^ rank' - 1) + 1 = 2 ^ rank' := by
+      grind
+    simp [h, pow_add]
+
+theorem init_unionFind.rankInvariant_strict {nodeList : List node} (h_nodup : nodeList.Nodup) : (init_unionFind nodeList h_nodup).rankInvariant_strict := by
+  simp [unionFind.rankInvariant_strict, init_unionFind, init_unionFind.linkList]
+  by_cases h_empty : nodeList = []
+  · simp [h_empty]
+  · simp [h_empty]
+    intro uFL h_in
+    have h_rank := init_unionFind.linkList.helper_all_rank_zero nodeList nodeList (by simp [h_empty]) uFL h_in
+    simp [h_rank]
+    have h_in_filter : uFL ∈ (List.filter (fun x => if h : x ∈ (init_unionFind nodeList h_nodup).linkList then decide (uFL ∈ get_parent_path (Eq.mpr_prop (Eq.refl (x ∈ (init_unionFind nodeList h_nodup).linkList)) h)) else false) (init_unionFind nodeList h_nodup).linkList) := by
+      simp [init_unionFind, init_unionFind.linkList, h_empty, h_in]
+      rw [get_parent_path]
+      split_ifs
+      · simp
+      · simp
+    have h_length : 1 ≤ (List.filter (fun x => if h : x ∈ (init_unionFind nodeList h_nodup).linkList then decide (uFL ∈ get_parent_path (Eq.mpr_prop (Eq.refl (x ∈ (init_unionFind nodeList h_nodup).linkList)) h)) else false) (init_unionFind nodeList h_nodup).linkList).length := by
+      grind
+    simp [init_unionFind, init_unionFind.linkList, h_empty] at h_length
+    exact h_length
+
+theorem update_unionFind.rankInvariant_strict {nodeList : List node} (uF : unionFind nodeList) (x y : ℕ) (h₁ : ∃ a ∈ uF.linkList, (fun a => a.nodeId = x ∧ a.ccId = x) a) (h₂ : ∃ a ∈ uF.linkList, (fun a => a.nodeId = y ∧ a.ccId = y) a) (h_rankInvariant : uF.rankInvariant_strict) : (update_unionFind uF x y h₁ h₂).rankInvariant_strict := by
+  simp [unionFind.rankInvariant_strict, update_unionFind]
+  set linklist' := (update_unionFind uF x y h₁ h₂).linkList with ← h_linklist'
+  set uFLx := List.choose (fun a => a.nodeId = x ∧ a.ccId = x) uF.linkList h₁ with ← h_uFLx
+  set uFLy := List.choose (fun a => a.nodeId = y ∧ a.ccId = y) uF.linkList h₂ with ← h_uFLy
+  have h_uFLx_in : uFLx ∈ uF.linkList := List.choose_mem (fun a => a.nodeId = x ∧ a.ccId = x) uF.linkList h₁
+  have h_uFLy_in : uFLy ∈ uF.linkList := List.choose_mem (fun a => a.nodeId = y ∧ a.ccId = y) uF.linkList h₂
+  have h_uFLx_prop : uFLx.nodeId = x ∧ uFLx.ccId = x := List.choose_property (fun a => a.nodeId = x ∧ a.ccId = x) uF.linkList h₁
+  have h_uFLy_prop : uFLy.nodeId = y ∧ uFLy.ccId = y := List.choose_property (fun a => a.nodeId = y ∧ a.ccId = y) uF.linkList h₂
+
+  simp [h_uFLx, h_uFLy]--, h_uFLy', h_linklist']
+  split_ifs with h_eq h_rank_lt'
+  · exact h_rankInvariant
+  -- wegen h_rank_lt kürzung
+  -- · set uFLx' : unionFindLink nodeList := { nodeId := uFLx.nodeId, ccId := uFLy.ccId, rank := uFLx.rank } with ← h_uFLx'
+  --   have h_rank_succ_le : uFLx.rank.val.succ ≤ uFLy.rank.val := by
+  --     simp [h_rank_lt]
+  --   have h_rank_succ_isLt : uFLx.rank.val.succ < nodeList.length := by
+  --     simp [Nat.lt_of_le_of_lt h_rank_succ_le]
+  --   set uFLy' : unionFindLink nodeList := { nodeId := uFLy.nodeId, ccId := uFLy.ccId, rank := ⟨max (uFLy.rank.val) (uFLx.rank.val + 1), by simp [h_rank_succ_isLt]⟩ } with ← h_uFLy'
+  --   simp [h_uFLy', h_uFLx']
+  --   simp [update_unionFind, h_uFLx, h_uFLy, h_uFLx', h_uFLy'] at h_linklist'
+  --   simp [h_eq, h_rank_lt] at h_linklist'
+  --   have h_uFLx'_in : uFLx' ∈ linklist' := by
+  --     simp [← h_linklist']
+  --     apply mem_set_of_ne_index
+  --     · apply List.mem_set
+  --       simp [List.idxOf_lt_length_iff, h_uFLx_in]
+  --     · have h : List.idxOf uFLx' (uF.linkList.set (List.idxOf uFLx uF.linkList) uFLx') = List.idxOf uFLx uF.linkList := by
+  --         apply idxOf_set
+  --         · intro j h_j
+  --           have h_not_in : ¬uFLx' ∈ uF.linkList := by
+  --             intro h_contra
+  --             have h := uF.matching_ccId uFLx h_uFLx_in
+  --             rcases h with ⟨z, h_z, _⟩
+  --             have h' := uF.matching_nodeId z h_z.left
+  --             rcases h' with ⟨w, h_w, h_unique⟩
+  --             simp [h_z.right] at h_unique
+  --             have h_eq1 := h_unique uFLx h_uFLx_in (by simp [h_uFLx_prop])
+  --             have h_eq2 := h_unique uFLx' h_contra (by simp [h_uFLx_prop, uFLx'])
+  --             grind
+  --           grind
+  --         · simp [List.idxOf_lt_length_iff, h_uFLx_in]
+  --       simp [h]
+  --       intro h_contra
+  --       have h : uFLx = uF.linkList[List.idxOf uFLx uF.linkList]'(by simp [List.idxOf_lt_length_iff, h_uFLx_in]) := by
+  --         simp
+  --       simp [h_contra] at h
+  --       simp [h, h_uFLy_prop] at h_uFLx_prop
+  --       simp [h_uFLx_prop] at h_eq
+  --   intro uFL h_uFL_in
+  --   simp [unionFind.rankInvariant_strict] at h_rankInvariant
+  --   by_cases h_uFL_eq : uFL = uFLx'
+  --   · have h := h_rankInvariant uFLx h_uFLx_in
+  --     set l1 := List.filter (fun x => if h : x ∈ uF.linkList then decide (uFLx ∈ get_parent_path h) else false) uF.linkList with ← h_l1
+  --     set l2 := List.filter (fun x_1 => if h : x_1 ∈ linklist' then decide (uFL ∈ get_parent_path h) else false) ((uF.linkList.set (List.idxOf uFLx uF.linkList) uFLx').set (List.idxOf uFLy uF.linkList) uFLy') with ← h_l2
+  --     simp [update_unionFind, linklist', h_eq, h_uFLx, h_uFLy, h_uFLx', h_uFLy'] at h_l2
+  --     simp [h_rank_lt] at h_l2
+  --     simp [h_l2]
+  --     simp [h_uFL_eq]
+  --     have h_rank_eq : 2 ^ uFLx'.rank.val = 2 ^ uFLx.rank.val := by
+  --       simp [uFLx']
+  --     apply le_of_eq_of_le h_rank_eq
+  --     apply le_trans h
+  --     let f : l1.toFinset → l2.toFinset := fun uFL1 =>
+  --       if h_uFL1_eq : uFL1 = uFLx
+  --         then
+  --           have h_uFLx'_in_finset : uFLx' ∈ l2.toFinset := by
+  --             simp [l2, h_uFLx'_in]
+  --             constructor
+  --             · simp [← h_linklist'] at h_uFLx'_in
+  --               exact h_uFLx'_in
+  --             · rw [get_parent_path]
+  --               grind
+  --           ⟨uFLx', h_uFLx'_in_finset⟩
+  --         else
+  --           have h_uFL1_in_finset : ↑uFL1 ∈ l2.toFinset := by
+  --             have h_uFL1_in := uFL1.mem
+  --             simp [l1] at h_uFL1_in
+  --             rcases h_uFL1_in with ⟨h_uFL1_in, h_uFL1_prop⟩
+  --             simp [l2]
+  --             constructor
+  --             · sorry
+  --             · sorry
+  --           ⟨uFL1, h_uFL1_in_finset⟩
+  --     apply nodup_length_le_length_of_injectiv_fun f
+  --     · exact List.Nodup.filter _ uF.nodup
+  --     · sorry
+  --   · sorry
+  · sorry
+  · sorry
+
+theorem max_rank {nodeList : List node} {uF : unionFind nodeList} (h_rankInvariant : uF.rankInvariant_strict) : ∀ uFL ∈ uF.linkList, uFL.rank.val ≤ Nat.log 2 nodeList.length := by
+  intro uFL h_uFL_in
+  by_cases h_contra : uFL.rank.val > Nat.log 2 nodeList.length
+  · simp [unionFind.rankInvariant_strict] at h_rankInvariant
+    have h := h_rankInvariant uFL h_uFL_in
+    have h : 2 ^ uFL.rank.val ≤ uF.linkList.length := by
+      apply le_trans h
+      simp [List.length_filter_le]
+    have h' : 2 ^ (Nat.log 2 nodeList.length + 1) ≤ 2 ^ uFL.rank.val := by
+      simp [Nat.pow_le_pow_iff_right]
+      exact h_contra
+    have h := le_trans h' h
+    simp [uF.matching_length.symm] at h
+    have h' := Nat.lt_pow_succ_log_self (b := 2) (by simp) nodeList.length
+    simp at h'
+    have h := lt_of_le_of_lt h h'
+    simp at h
+  · simp at h_contra
+    exact h_contra
+
+-- theorem SimpleGraph_of_kruskal_IsEqReachable (edgeList : List edge) (h : edgeList ≠ []) : ∀ (x y), (SimpleGraph_of_edgeList edgeList h).Reachable x y ↔ (SimpleGraph_of_kruskal edgeList h).Reachable x y := by sorry
+
+-- theorem SimpleGraph_of_kruskal_IsSpanningTree (edgeList : List edge) (h : edgeList ≠ []) : SimpleGraph.IsSpanningTree (SimpleGraph_of_kruskal edgeList h) (SimpleGraph_of_edgeList edgeList h) := by sorry
+
+def cost_of_edgeList : List edge → Nat
+  | [] => 0
+  | e :: edgeList => e.cost + cost_of_edgeList edgeList
+
+-- def minimalSpanninTree_of_edgeList (edgeList : List edge) (h₁ : edgeList ≠ []) (G := SimpleGraph_of_edgeList edgeList h₁) (minEdgeList : List edge) (h₂ : minEdgeList ≠ []) (h₃ : SimpleGraph.IsSpanningTree G (SimpleGraph_of_edgeList minEdgeList h₂)) (h₄ : ∀ x ∈ minEdgeList, x ∈ edgeList) : Prop := ∀ (el : List edge), (h₅ : el ≠ []) → (h₆ : ∀ x ∈ el, x ∈ edgeList) → SimpleGraph.IsSpanningTree G (SimpleGraph_of_edgeList el h₅) → (cost_of_edgeList el) ≥ (cost_of_edgeList minEdgeList)
+
+-- theorem kruskal_minimalSpanninTree_of_edgeList (edgeList : List edge) (h : edgeList ≠ []) : minimalSpanninTree_of_edgeList edgeList h (SimpleGraph_of_edgeList edgeList h₁) (kruskal_of_edgeList edgeList) (kruskal_nonempty edgeList h) := by sorry
+
+-- #min_imports
